<?xml version="1.0"?>
<rdf:RDF xmlns="http://example.org/techLayer2#"
     xml:base="http://example.org/techLayer2"
     xmlns:rdf="http://www.w3.org/1999/02/22-rdf-syntax-ns#"
     xmlns:owl="http://www.w3.org/2002/07/owl#"
     xmlns:rdfs="http://www.w3.org/2000/01/rdf-schema#"
     xmlns:xsd="http://www.w3.org/2001/XMLSchema#">

     <!-- ********************************************************************************************* -->
     <!-- *******************  All rights reserved to Cristian Lepore ********************************* -->
     <!-- ************************* Tech layer 2 of the ToIP model ************************************ -->
     <!-- ******** Definitions comes from the ToIP Glossary: https://glossary.trustoverip.org/ ******** -->
     <!-- ********************************************************************************************* -->

     <owl:Ontology rdf:about="http://example.org/techLayer2#">
          <rdfs:comment>Ontology representing the tech Layer 2 of the ToIP stack.</rdfs:comment>
     </owl:Ontology>



     <!-- ******************************* -->
     <!-- ********* Class *************** -->
     <!-- ******************************* -->

     <owl:Class rdf:about="techLayer2#IntermediarySystem">
          <rdfs:label>Intermediary System</rdfs:label>
          <rdfs:comment>An intermediary system routes messages between endpoint systems but is not otherwise involved in the processing of those messages. In the context of end-to-end encryption, intermediary systems cannot decrypt the messages sent between the endpoint systems. In the ToIP stack, intermediary systems operate at ToIP Layer 2, the trust spanning layer. An intermediary system is one of three types of systems defined in the ToIP Technology Architecture Specification; the other two are endpoint systems and supporting systems.</rdfs:comment>
          <rdfs:isDefinedBy rdf:resource="https://glossary.trustoverip.org/#term:intermediary-system"/>
     </owl:Class>

     <owl:Class rdf:about="techLayer2#ThirdParty">
          <rdfs:label>Third party</rdfs:label>
          <rdfs:comment>A party that is not directly involved in the trust relationship between a first party and a second party, but provides supporting services to either or both of them.</rdfs:comment>
          <rdfs:subClassOf rdf:resource="techLayer2#IntermediarySystem"/>
          <rdfs:isDefinedBy rdf:resource="https://glossary.trustoverip.org/#term:third-party"/>
     </owl:Class>



     <!-- ******************************* -->
     <!-- ********* Attribute *********** -->
     <!-- ******************************* -->

     <owl:DatatypeProperty rdf:about="techLayer2#edgeAgent">
          <rdfs:domain rdf:resource="techLayer2#UserAgent"/>
          <rdfs:range rdf:resource="http://www.w3.org/2001/XMLSchema#boolean"/>
          <rdfs:label>edge</rdfs:label>
          <rdfs:comment></rdfs:comment>
          <rdfs:isDefinedBy rdf:resource=""/>
     </owl:DatatypeProperty>

     <owl:DatatypeProperty rdf:about="techLayer2#cloudDataVault">
          <rdfs:domain rdf:resource="techLayer2#DataVault"/>
          <rdfs:range rdf:resource="http://www.w3.org/2001/XMLSchema#boolean"/>
          <rdfs:label>cloud</rdfs:label>
          <rdfs:comment>A digital vault may be implemented on a local device or in the cloud.</rdfs:comment>
          <rdfs:isDefinedBy rdf:resource="https://glossary.trustoverip.org/#term:digital-vault"/>
     </owl:DatatypeProperty>



     <!-- ******************************* -->
     <!-- ********* Relation ************ -->
     <!-- ******************************* -->

     <owl:ObjectProperty rdf:about="techLayer2#ExternalBackup">
          <rdfs:domain rdf:resource="techLayer2#DataVault"/>
          <rdfs:range rdf:resource="techLayer2#ThirdParty"/>
          <rdfs:label>backs up</rdfs:label>
     </owl:ObjectProperty>

     <owl:ObjectProperty rdf:about="techLayer2#hasDataVault">
          <rdfs:domain rdf:resource="techLayer2#UserAgent"/>
          <rdfs:range rdf:resource="techLayer2#DataVault"/>
          <rdfs:label>has</rdfs:label>
          <rdfs:comment>A secure container for data whose controller is the principal. A digital vault is most commonly used in conjunction with a digital wallet and a digital agent. A digital vault may be implemented on a local device or in the cloud; multiple digital vaults may be used by the same principal across different devices and/or the cloud; if so they may use some type of synchronization. If the capability is supported, data may flow into or out of the digital vault automatically based on subscriptions approved by the controller.</rdfs:comment>
          <rdfs:isDefinedBy rdf:resource="https://glossary.trustoverip.org/#term:data-vault"/>
     </owl:ObjectProperty>




     <!-- ******************************* -->
     <!-- * Connection with other Layer * -->
     <!-- ******************************* -->

     <owl:Class rdf:about="techLayer3#Credential">
          <rdfs:label>Credential</rdfs:label>
          <rdfs:comment>A container of claims describing one or more subjects. A credential is generated by the issuer of the credential and given to the holder of the credential. A credential typically includes a signature or some other means of proving its authenticity. A credential may be either a physical credential or a digital credential.</rdfs:comment>
          <rdfs:isDefinedBy rdf:resource="https://glossary.trustoverip.org/#term:credential"/>
     </owl:Class>



     <!-- ******************************* -->
     <!-- ********* Instance ************ -->
     <!-- ******************************* -->



</rdf:RDF>
