<?xml version="1.0"?>
<rdf:RDF xmlns="http://example.org/techLayer2#"
     xml:base="http://example.org/techLayer2"
     xmlns:rdf="http://www.w3.org/1999/02/22-rdf-syntax-ns#"
     xmlns:owl="http://www.w3.org/2002/07/owl#"
     xmlns:rdfs="http://www.w3.org/2000/01/rdf-schema#"
     xmlns:xsd="http://www.w3.org/2001/XMLSchema#">

     <!-- ********************************************************************************************* -->
     <!-- *******************  All rights reserved to Cristian Lepore ********************************* -->
     <!-- ************************* Tech layer 2 of the ToIP model ************************************ -->
     <!-- ******** Definitions comes from the ToIP Glossary: https://glossary.trustoverip.org/ ******** -->
     <!-- ********************************************************************************************* -->

     <owl:Ontology rdf:about="http://example.org/techLayer2#">
          <rdfs:comment>Ontology representing the tech Layer 2 of the ToIP stack.</rdfs:comment>
     </owl:Ontology>



     <!-- ******************************* -->
     <!-- ********* Class *************** -->
     <!-- ******************************* -->

     <owl:Class rdf:about="techLayer2#UserAgent">
          <rdfs:label>User Agent</rdfs:label>
          <rdfs:comment>A software agent that is used directly by the end-user as the principal. Browsers, email clients, and digital wallets are all examples of user agents.</rdfs:comment>
          <rdfs:isDefinedBy rdf:resource="https://glossary.trustoverip.org/#term:user-agent"/>
     </owl:Class>

     <owl:Class rdf:about="techLayer2#DataVault">
          <rdfs:label>Data vault</rdfs:label>
          <rdfs:comment>A secure container for data whose controller is the principal. A digital vault is most commonly used in conjunction with a digital wallet and a digital agent. A digital vault may be implemented on a local device or in the cloud; multiple digital vaults may be used by the same principal across different devices and/or the cloud; if so they may use some type of synchronization. If the capability is supported, data may flow into or out of the digital vault automatically based on subscriptions approved by the controller.</rdfs:comment>
          <rdfs:isDefinedBy rdf:resource="https://glossary.trustoverip.org/#term:data-vault"/>
     </owl:Class>

     <owl:Class rdf:about="techLayer2#KeyManagementSystem">
          <rdfs:label>Key management system</rdfs:label>
          <rdfs:comment>A system for the management of cryptographic keys and their metadata (e.g., generation, distribution, storage, backup, archive, recovery, use, revocation, and destruction). An automated key management system may be used to oversee, automate, and secure the key management process. A key management is often protected by implementing it within the trusted execution environment (TEE) of a device. An example is the Secure Enclave on Apple iOS devices.</rdfs:comment>
          <rdfs:isDefinedBy rdf:resource="https://glossary.trustoverip.org/#term:key-management-system"/>
     </owl:Class>

     <owl:Class rdf:about="techLayer2#TrustedCommunicationProtocol">
          <rdfs:label>Trusted Communication Protocol</rdfs:label>
          <rdfs:comment>The ToIP Trust Spanning Protocol (TSP) is the ToIP Layer 2 protocol for verifiable messaging that implements the trust spanning layer of the ToIP stack.  The TSP enables actors in different digital trust domains to interact in a similar way to how the Internet Protocol (IP) enables devices on different local area networks to exchange data.</rdfs:comment>
          <rdfs:isDefinedBy rdf:resource="https://glossary.trustoverip.org/#term:toip-trust-spanning-protocol"/>
     </owl:Class>

     <owl:Class rdf:about="techLayer2#IntermediarySystem">
          <rdfs:label>Intermediary System</rdfs:label>
          <rdfs:comment>An intermediary system routes messages between endpoint systems but is not otherwise involved in the processing of those messages. In the context of end-to-end encryption, intermediary systems cannot decrypt the messages sent between the endpoint systems. In the ToIP stack, intermediary systems operate at ToIP Layer 2, the trust spanning layer. An intermediary system is one of three types of systems defined in the ToIP Technology Architecture Specification; the other two are endpoint systems and supporting systems.</rdfs:comment>
          <rdfs:isDefinedBy rdf:resource="https://glossary.trustoverip.org/#term:intermediary-system"/>
     </owl:Class>

     <owl:Class rdf:about="techLayer2#ThirdParty">
          <rdfs:label>Third party</rdfs:label>
          <rdfs:comment>A party that is not directly involved in the trust relationship between a first party and a second party, but provides supporting services to either or both of them.</rdfs:comment>
          <rdfs:subClassOf rdf:resource="techLayer2#IntermediarySystem"/>
          <rdfs:isDefinedBy rdf:resource="https://glossary.trustoverip.org/#term:third-party"/>
     </owl:Class>

     <owl:Class rdf:about="techLayer2#AuthenticationProtocol">
          <rdfs:label>Authentication protocol</rdfs:label>
          <rdfs:comment>Verifying the identity of a user, process, or device, often as a prerequisite to allowing access to resources in an information system.</rdfs:comment>
          <rdfs:subClassOf rdf:resource="techLayer2#TrustedCommunicationProtocol"/>
          <rdfs:isDefinedBy rdf:resource="https://glossary.trustoverip.org/#term:authentication"/>
     </owl:Class>

     <owl:Class rdf:about="techLayer2#EncryptionProtocol">
          <rdfs:label>Encryption protocol</rdfs:label>
          <rdfs:comment>Encryption that is applied to a communication before it is transmitted from the sender's communication endpoint and cannot be decrypted until after it is received at the receiver's communication endpoint. When end-to-end encryption is used, the communication cannot be decrypted in transit no matter how many intermediaries are involved in the routing process.</rdfs:comment>
          <rdfs:subClassOf rdf:resource="techLayer2#AuthenticationProtocol"/>
          <rdfs:isDefinedBy rdf:resource="https://glossary.trustoverip.org/#term:end-to-end-encryption"/>
     </owl:Class>



     <!-- ******************************* -->
     <!-- ********* Attribute *********** -->
     <!-- ******************************* -->

     <owl:DatatypeProperty rdf:about="techLayer2#edgeAgent">
          <rdfs:domain rdf:resource="techLayer2#UserAgent"/>
          <rdfs:range rdf:resource="http://www.w3.org/2001/XMLSchema#boolean"/>
          <rdfs:label>edge</rdfs:label>
          <rdfs:comment></rdfs:comment>
          <rdfs:isDefinedBy rdf:resource=""/>
     </owl:DatatypeProperty>

     <owl:DatatypeProperty rdf:about="techLayer2#cloudAgent">
          <rdfs:domain rdf:resource="techLayer2#UserAgent"/>
          <rdfs:range rdf:resource="http://www.w3.org/2001/XMLSchema#boolean"/>
          <rdfs:label>cloud</rdfs:label>
          <rdfs:comment></rdfs:comment>
          <rdfs:isDefinedBy rdf:resource=""/>
     </owl:DatatypeProperty>

     <owl:DatatypeProperty rdf:about="techLayer2#localDataVault">
          <rdfs:domain rdf:resource="techLayer2#DataVault"/>
          <rdfs:range rdf:resource="http://www.w3.org/2001/XMLSchema#boolean"/>
          <rdfs:label>local</rdfs:label>
          <rdfs:comment>A digital vault may be implemented on a local device or in the cloud.</rdfs:comment>
          <rdfs:isDefinedBy rdf:resource="https://glossary.trustoverip.org/#term:digital-vault"/>
     </owl:DatatypeProperty>

     <owl:DatatypeProperty rdf:about="techLayer2#cloudDataVault">
          <rdfs:domain rdf:resource="techLayer2#DataVault"/>
          <rdfs:range rdf:resource="http://www.w3.org/2001/XMLSchema#boolean"/>
          <rdfs:label>cloud</rdfs:label>
          <rdfs:comment>A digital vault may be implemented on a local device or in the cloud.</rdfs:comment>
          <rdfs:isDefinedBy rdf:resource="https://glossary.trustoverip.org/#term:digital-vault"/>
     </owl:DatatypeProperty>



     <!-- ******************************* -->
     <!-- ********* Relation ************ -->
     <!-- ******************************* -->

     <owl:ObjectProperty rdf:about="techLayer2#ExternalBackup">
          <rdfs:domain rdf:resource="techLayer2#DataVault"/>
          <rdfs:range rdf:resource="techLayer2#ThirdParty"/>
          <rdfs:label>backs up</rdfs:label>
     </owl:ObjectProperty>

     <owl:ObjectProperty rdf:about="techLayer2#enablesTSP">
          <rdfs:domain rdf:resource="techLayer2#UserAgent"/>
          <rdfs:range rdf:resource="techLayer2#TrustedCommunicationProtocol"/>
          <rdfs:label>enables</rdfs:label>
          <rdfs:comment>The endpoint sends and receives messages using the Trusted Communication Protocol.</rdfs:comment>
     </owl:ObjectProperty>

     <owl:ObjectProperty rdf:about="techLayer2#storesIdentifier">
          <rdfs:domain rdf:resource="techLayer2#DataVault"/>
          <rdfs:range rdf:resource="techLayer1#Identifier"/>
          <rdfs:label>stores</rdfs:label>
          <rdfs:comment>The endpoint sends and receives messages using the Trusted Communication Protocol.</rdfs:comment>
     </owl:ObjectProperty>

     <owl:ObjectProperty rdf:about="techLayer2#LocalBackup">
          <rdfs:domain rdf:resource="techLayer2#DataVault"/>
          <rdfs:range rdf:resource="techLayer2#DataVault"/>
          <rdfs:label>backs up</rdfs:label>
     </owl:ObjectProperty>

     <owl:ObjectProperty rdf:about="techLayer2#hasKeyManagementSystem">
          <rdfs:domain rdf:resource="techLayer2#UserAgent"/>
          <rdfs:range rdf:resource="techLayer2#KeyManagementSystem"/>
          <rdfs:label>has</rdfs:label>
          <rdfs:comment>A system for the management of cryptographic keys and their metadata (e.g., generation, distribution, storage, backup, archive, recovery, use, revocation, and destruction). An automated key management system may be used to oversee, automate, and secure the key management process. A key management is often protected by implementing it within the trusted execution environment (TEE) of a device. An example is the Secure Enclave on Apple iOS devices.</rdfs:comment>
          <rdfs:isDefinedBy rdf:resource="https://glossary.trustoverip.org/#term:key-management-system"/>
     </owl:ObjectProperty>

     <owl:ObjectProperty rdf:about="techLayer2#hasDataVault">
          <rdfs:domain rdf:resource="techLayer2#UserAgent"/>
          <rdfs:range rdf:resource="techLayer2#DataVault"/>
          <rdfs:label>has</rdfs:label>
          <rdfs:comment>A secure container for data whose controller is the principal. A digital vault is most commonly used in conjunction with a digital wallet and a digital agent. A digital vault may be implemented on a local device or in the cloud; multiple digital vaults may be used by the same principal across different devices and/or the cloud; if so they may use some type of synchronization. If the capability is supported, data may flow into or out of the digital vault automatically based on subscriptions approved by the controller.</rdfs:comment>
          <rdfs:isDefinedBy rdf:resource="https://glossary.trustoverip.org/#term:data-vault"/>
     </owl:ObjectProperty>

     <owl:ObjectProperty rdf:about="techLayer2#managesIdentifier">
          <rdfs:domain rdf:resource="techLayer2#KeyManagementSystem"/>
          <rdfs:range rdf:resource="techLayer1#Identifier"/>
          <rdfs:label>manages</rdfs:label>
          <rdfs:comment>A system for the management of cryptographic keys and their metadata (e.g., generation, distribution, storage, backup, archive, recovery, use, revocation, and destruction). An automated key management system may be used to oversee, automate, and secure the key management process. A key management is often protected by implementing it within the trusted execution environment (TEE) of a device. An example is the Secure Enclave on Apple iOS devices.</rdfs:comment>
          <rdfs:isDefinedBy rdf:resource="https://glossary.trustoverip.org/#term:key-management-system"/>
     </owl:ObjectProperty>

     <owl:ObjectProperty rdf:about="techLayer2#maintainsCredential">
          <rdfs:domain rdf:resource="techLayer2#DataVault"/>
          <rdfs:range rdf:resource="techLayer3#Credential"/>
          <rdfs:label>maintains</rdfs:label>
          <rdfs:comment>A secure container for data whose controller is the principal. A digital vault is most commonly used in conjunction with a digital wallet and a digital agent. A digital vault may be implemented on a local device or in the cloud; multiple digital vaults may be used by the same principal across different devices and/or the cloud; if so they may use some type of synchronization. If the capability is supported, data may flow into or out of the digital vault automatically based on subscriptions approved by the controller.</rdfs:comment>
          <rdfs:isDefinedBy rdf:resource="https://glossary.trustoverip.org/#term:data-vault"/>
     </owl:ObjectProperty>

     <owl:ObjectProperty rdf:about="techLayer2#routesThroughIntermediarySystem">
          <rdfs:domain rdf:resource="techLayer2#TrustedCommunicationProtocol"/>
          <rdfs:range rdf:resource="techLayer2#IntermediarySystem"/>
          <rdfs:label>routes through</rdfs:label>
          <rdfs:comment>An intermediary system routes messages between endpoint systems but is not otherwise involved in the processing of those messages. In the context of end-to-end encryption, intermediary systems cannot decrypt the messages sent between the endpoint systems. In the ToIP stack, intermediary systems operate at ToIP Layer 2, the trust spanning layer. An intermediary system is one of three types of systems defined in the ToIP Technology Architecture Specification; the other two are endpoint systems and supporting systems.</rdfs:comment>
          <rdfs:isDefinedBy rdf:resource="https://glossary.trustoverip.org/#term:intermediary-system"/>
     </owl:ObjectProperty>



     <!-- ******************************* -->
     <!-- * Connection with other Layer * -->
     <!-- ******************************* -->

     <owl:Class rdf:about="techLayer3#Credential">
          <rdfs:label>Credential</rdfs:label>
          <rdfs:comment>A container of claims describing one or more subjects. A credential is generated by the issuer of the credential and given to the holder of the credential. A credential typically includes a signature or some other means of proving its authenticity. A credential may be either a physical credential or a digital credential.</rdfs:comment>
          <rdfs:isDefinedBy rdf:resource="https://glossary.trustoverip.org/#term:credential"/>
     </owl:Class>

     <owl:Class rdf:about="techLayer1#Identifier">
          <rdfs:label>Identifier</rdfs:label>
          <rdfs:comment>A single attribute—typically a character string—that uniquely identifies an entity within a specific context (which may be a global context). Examples include the name of a party, the URL of an organization, or a serial number for a man-made thing.</rdfs:comment>
          <rdfs:subClassOf rdf:resource="techLayer1#DigitalTrustUtility"/>
          <rdfs:isDefinedBy rdf:resource="https://glossary.trustoverip.org/#term:identifier"/>
     </owl:Class>



     <!-- ******************************* -->
     <!-- ********* Instance ************ -->
     <!-- ******************************* -->



</rdf:RDF>
