<?xml version="1.0"?>
<rdf:RDF xmlns="http://example.org/governance#"
    xml:base="http://example.org/governance"
    xmlns:rdf="http://www.w3.org/1999/02/22-rdf-syntax-ns#"
    xmlns:owl="http://www.w3.org/2002/07/owl#"
    xmlns:rdfs="http://www.w3.org/2000/01/rdf-schema#"
    xmlns:xsd="http://www.w3.org/2001/XMLSchema#">



    <!-- ********************************************************************************************* -->
    <!-- *******************  All rights reserved to Cristian Lepore ********************************* -->
    <!-- ************************* Governance of the ToIP model ************************************** -->
    <!-- ******** Definitions comes from the ToIP Glossary: https://glossary.trustoverip.org/ ******** -->
    <!-- ********************************************************************************************* -->

    <owl:Ontology rdf:about="http://example.org/governance#">
        <rdfs:comment>Ontology representing the governance of the ToIP stack.</rdfs:comment>
    </owl:Ontology>



    <!-- ******************************* -->
    <!-- ********* Class *************** -->
    <!-- ******************************* -->

    <owl:Class rdf:about="governance#GoverningAuthority">
        <rdfs:label>Governing authority</rdfs:label>
        <rdfs:comment>The party (or set of parties) authoritative for governing a trust community, usually (but not always) by developing, publishing, maintaining, and enforcing a governance framework. A governing body may be a government, a formal legal entity of any kind, an informal group of any kind, or an individual. A governing body may also delegate operational responsibilities to an administering body.</rdfs:comment>
        <rdfs:subClassOf rdf:resource="techLayer4#Entity"/>
        <rdfs:isDefinedBy rdf:resource="https://glossary.trustoverip.org/#term:governing-authority"/>
    </owl:Class>

    <owl:Class rdf:about="governance#AdministeringAuthority">
        <rdfs:label>Administering authority</rdfs:label>
        <rdfs:comment>A legal entity delegated by a governing body to administer the operation of a governance framework and governed infrastructure for a digital trust ecosystem, such as one or more trust registries.</rdfs:comment>
        <rdfs:subClassOf rdf:resource="techLayer4#Entity"/>
        <rdfs:isDefinedBy rdf:resource="https://glossary.trustoverip.org/#term:administering-authority"/>
    </owl:Class>

    <owl:Class rdf:about="governance#GovernanceFramework">
        <rdfs:label>Governance framework</rdfs:label>
        <rdfs:comment>A collection of one or more governance documents published by the governing body of a trust community.</rdfs:comment>
        <rdfs:isDefinedBy rdf:resource="https://glossary.trustoverip.org/#term:governance-framework"/>
    </owl:Class>

    <owl:Class rdf:about="governance#GovernanceDocument">
        <rdfs:label>Governance document</rdfs:label>
        <rdfs:comment>A document with at least one identifier that specifies governance requirements for a trust community. Note: A governance document is a component of a governance framework.</rdfs:comment>
        <rdfs:subClassOf rdf:resource="governance#GovernanceFramework"/>
        <rdfs:isDefinedBy rdf:resource="https://glossary.trustoverip.org/#term:governance-document"/>
    </owl:Class>

    <owl:Class rdf:about="governance#PrimaryDocument">
        <rdfs:label>Primary document</rdfs:label>
        <rdfs:comment>The governance document at the root of a governance framework. The primary document specifies the other controlled documents in the governance framework.</rdfs:comment>
        <rdfs:subClassOf rdf:resource="governance#GovernanceDocument"/>
        <rdfs:isDefinedBy rdf:resource="https://glossary.trustoverip.org/#term:primary-document"/>
    </owl:Class>

    <owl:Class rdf:about="governance#ControlledDocument">
        <rdfs:label>Controlled document</rdfs:label>
        <rdfs:comment>A governance document whose authority is derived from a primary document.</rdfs:comment>
        <rdfs:subClassOf rdf:resource="governance#GovernanceDocument"/>
        <rdfs:isDefinedBy rdf:resource="https://glossary.trustoverip.org/#term:controlled-document"/>
    </owl:Class>

    <owl:Class rdf:about="governance#SectorSpecificPolicy">
        <rdfs:label>Sector-specific policy</rdfs:label>
        <rdfs:comment>Statements,rules, or assertions that specify the correct or expected behavior of an entity. For example, an authorization policy might specify the correct access control rules for a software component. Policies may be human-readable or machine-readable or both.</rdfs:comment>
        <rdfs:isDefinedBy rdf:resource="https://glossary.trustoverip.org/#term:policy"/>
    </owl:Class>

    <owl:Class rdf:about="governance#LegalAgreement">
        <rdfs:label>Legal agreement</rdfs:label>
        <rdfs:subClassOf rdf:resource="governance#GovernanceDocument"/>
        <rdfs:isDefinedBy rdf:resource="https://sovrin.org/wp-content/uploads/Sovrin-Governance-Framework-V2-Master-Document-V2.pdf"/>
    </owl:Class>

    <owl:Class rdf:about="governance#Definition">
        <rdfs:label>Definition</rdfs:label>
        <rdfs:subClassOf rdf:resource="governance#ControlledDocument"/>
        <rdfs:isDefinedBy rdf:resource="https://sovrin.org/wp-content/uploads/Sovrin-Governance-Framework-V2-Master-Document-V2.pdf"/>
    </owl:Class>

    <owl:Class rdf:about="governance#Specification">
        <rdfs:label>Specification</rdfs:label>
        <rdfs:subClassOf rdf:resource="governance#ControlledDocument"/>
        <rdfs:isDefinedBy rdf:resource="https://sovrin.org/wp-content/uploads/Sovrin-Governance-Framework-V2-Master-Document-V2.pdf"/>
    </owl:Class>

    <owl:Class rdf:about="governance#Policy">
        <rdfs:label>Policy</rdfs:label>
        <rdfs:subClassOf rdf:resource="governance#ControlledDocument"/>
        <rdfs:isDefinedBy rdf:resource="https://sovrin.org/wp-content/uploads/Sovrin-Governance-Framework-V2-Master-Document-V2.pdf"/>
    </owl:Class>

    <owl:Class rdf:about="governance#Framework">
        <rdfs:label>Framework</rdfs:label>
        <rdfs:subClassOf rdf:resource="governance#ControlledDocument"/>
        <rdfs:isDefinedBy rdf:resource="https://sovrin.org/wp-content/uploads/Sovrin-Governance-Framework-V2-Master-Document-V2.pdf"/>
    </owl:Class>



    <!-- ******************************* -->
    <!-- ********* Relation ************ -->
    <!-- ******************************* -->

    <owl:ObjectProperty rdf:about="governance#enforcesGovernanceFramework">
        <rdfs:domain rdf:resource="governance#GoverningAuthority"/>
        <rdfs:range rdf:resource="governance#GovernanceFramework"/>
        <rdfs:label>enforces</rdfs:label>
        <rdfs:comment>The party (or set of parties) authoritative for governing a trust community, usually (but not always) by developing, publishing, maintaining, and enforcing a governance framework. A governing body may be a government, a formal legal entity of any kind, an informal group of any kind, or an individual. A governing body may also delegate operational responsibilities to an administering body.</rdfs:comment>
        <rdfs:isDefinedBy rdf:resource="https://glossary.trustoverip.org/#term:governing-authority"/>
    </owl:ObjectProperty>

    <owl:ObjectProperty rdf:about="governance#hasIdentifier">
        <rdfs:domain rdf:resource="governance#GovernanceDocument"/>
        <rdfs:range rdf:resource="techLayer1#Identifier"/>
        <rdfs:label>has</rdfs:label>
        <rdfs:comment>A document with at least one identifier that specifies governance requirements for a trust community. Note: A governance document is a component of a governance framework.</rdfs:comment>
        <rdfs:isDefinedBy rdf:resource="https://glossary.trustoverip.org/#term:governance-document"/>
    </owl:ObjectProperty>

    <owl:ObjectProperty rdf:about="governance#delegatesAdministeringAuthority">
        <rdfs:domain rdf:resource="governance#GoverningAuthority"/>
        <rdfs:range rdf:resource="governance#AdministeringAuthority"/>
        <rdfs:label>delegates</rdfs:label>
        <rdfs:comment>The party (or set of parties) authoritative for governing a trust community, usually (but not always) by developing, publishing, maintaining, and enforcing a governance framework. A governing body may be a government, a formal legal entity of any kind, an informal group of any kind, or an individual. A governing body may also delegate operational responsibilities to an administering body.</rdfs:comment>
        <rdfs:isDefinedBy rdf:resource="https://glossary.trustoverip.org/#term:governing-authority"/>
    </owl:ObjectProperty>

    <owl:ObjectProperty rdf:about="governance#administersDigitalTrustUtility">
        <rdfs:domain rdf:resource="governance#AdministeringAuthority"/>
        <rdfs:range rdf:resource="techLayer1#DigitalTrustUtility"/>
        <rdfs:label>administers</rdfs:label>
        <rdfs:comment>A legal entity delegated by a governing body to administer the operation of a governance framework and governed infrastructure for a digital trust ecosystem, such as one or more trust registries.</rdfs:comment>
        <rdfs:isDefinedBy rdf:resource="https://glossary.trustoverip.org/#term:administering-authority"/>
    </owl:ObjectProperty>

    <owl:ObjectProperty rdf:about="governance#specifiesControlledDocument">
        <rdfs:domain rdf:resource="governance#PrimaryDocument"/>
        <rdfs:range rdf:resource="governance#ControlledDocument"/>
        <rdfs:label>specifies</rdfs:label>
        <rdfs:comment>The governance document at the root of a governance framework. The primary document specifies the other controlled documents in the governance framework.</rdfs:comment>
        <rdfs:isDefinedBy rdf:resource="https://glossary.trustoverip.org/#term:primary-document"/>
    </owl:ObjectProperty>

    <owl:ObjectProperty rdf:about="governance#complementsSectorSpecificPolicy">
        <rdfs:domain rdf:resource="governance#SectorSpecificPolicy"/>
        <rdfs:range rdf:resource="governance#GovernanceFramework"/>
        <rdfs:label>complements</rdfs:label>
        <rdfs:comment>The governance is a layering approach, with sector-specific policies that complemente the national identity policy. (from the ToIP document of mapping ToIP with the Bhutan national identity framework)</rdfs:comment>
    </owl:ObjectProperty>

    <owl:ObjectProperty rdf:about="governance#interactsWithAdministeringAuthority">
        <rdfs:domain rdf:resource="governance#AdministeringAuthority"/>
        <rdfs:range rdf:resource="governance#AdministeringAuthority"/>
        <rdfs:label>interacts</rdfs:label>
        <rdfs:comment>The entity in a public key infrastructure (PKI) that is responsible for issuing public key certificates and exacting compliance to a PKI policy.</rdfs:comment>
        <rdfs:isDefinedBy rdf:resource="https://glossary.trustoverip.org/#term:certificate-authority"/>
    </owl:ObjectProperty>

    <owl:ObjectProperty rdf:about="governance#rulesParty">
        <rdfs:domain rdf:resource="governance#GovernanceFramework"/>
        <rdfs:range rdf:resource="techLayer4#TrustCommunity"/>
        <rdfs:label>rules</rdfs:label>
        <rdfs:comment>The governance framework rules the parties.</rdfs:comment>
        <rdfs:isDefinedBy rdf:resource=""/>
    </owl:ObjectProperty>



    <!-- ******************************* -->
    <!-- ********* Attribute *********** -->
    <!-- ******************************* -->

    <owl:DatatypeProperty rdf:about="governance#formal">
        <rdfs:domain rdf:resource="governance#GovernanceFramework"/>
        <rdfs:range rdf:resource="http://www.w3.org/2001/XMLSchema#boolean"/>
        <rdfs:label>formal</rdfs:label>
        <rdfs:comment>Indicates whether the governance framework is formal.</rdfs:comment>
    </owl:DatatypeProperty>

    <owl:ObjectProperty rdf:about="techLayer4#memberOfTrustCommunity">
        <rdfs:domain rdf:resource="techLayer4#Entity"/>
        <rdfs:range rdf:resource="techLayer4#TrustCommunity"/>
        <rdfs:label>member</rdfs:label>
    </owl:ObjectProperty>

    <owl:DatatypeProperty rdf:about="governance#open">
        <rdfs:domain rdf:resource="governance#GovernanceFramework"/>
        <rdfs:range rdf:resource="http://www.w3.org/2001/XMLSchema#boolean"/>
        <rdfs:label>open</rdfs:label>
        <rdfs:comment>Indicates whether the governance framework is open to public review and comment.</rdfs:comment>
    </owl:DatatypeProperty>

    <owl:DatatypeProperty rdf:about="governance#informal">
        <rdfs:domain rdf:resource="governance#GovernanceFramework"/>
        <rdfs:range rdf:resource="http://www.w3.org/2001/XMLSchema#boolean"/>
        <rdfs:label>informal</rdfs:label>
        <rdfs:comment>Indicates whether the governance framework is informal.</rdfs:comment>
    </owl:DatatypeProperty>

    <owl:DatatypeProperty rdf:about="governance#manual">
        <rdfs:domain rdf:resource="governance#GovernanceFramework"/>
        <rdfs:range rdf:resource="http://www.w3.org/2001/XMLSchema#boolean"/>
        <rdfs:label>manual</rdfs:label>
        <rdfs:comment>Indicates whether the governance framework is manual.</rdfs:comment>
    </owl:DatatypeProperty>
    
    <owl:DatatypeProperty rdf:about="governance#algorithmic">
        <rdfs:domain rdf:resource="governance#GovernanceFramework"/>
        <rdfs:range rdf:resource="http://www.w3.org/2001/XMLSchema#boolean"/>
        <rdfs:label>algorithmic</rdfs:label>
        <rdfs:comment>Indicates whether the governance framework is Algorithmic.</rdfs:comment>
    </owl:DatatypeProperty>

    <owl:DatatypeProperty rdf:about="governance#centralized">
        <rdfs:domain rdf:resource="governance#GoverningAuthority"/>
        <rdfs:range rdf:resource="http://www.w3.org/2001/XMLSchema#boolean"/>
        <rdfs:label>centralized</rdfs:label>
        <rdfs:comment>Indicates whether the governing is centralized.</rdfs:comment>
    </owl:DatatypeProperty>

    <owl:DatatypeProperty rdf:about="governance#decentralized">
        <rdfs:domain rdf:resource="governance#GoverningAuthority"/>
        <rdfs:range rdf:resource="http://www.w3.org/2001/XMLSchema#boolean"/>
        <rdfs:label>decentralized</rdfs:label>
        <rdfs:comment>Indicates whether the governing is decentralized.</rdfs:comment>
    </owl:DatatypeProperty>

    <owl:DatatypeProperty rdf:about="governance#federated">
        <rdfs:domain rdf:resource="governance#GoverningAuthority"/>
        <rdfs:range rdf:resource="http://www.w3.org/2001/XMLSchema#boolean"/>
        <rdfs:label>federated</rdfs:label>
        <rdfs:comment>Indicates whether the governing is federated.</rdfs:comment>
    </owl:DatatypeProperty>
     


    <!-- ******************************* -->
    <!-- * Connection with other Layer * -->
    <!-- ******************************* -->

    <owl:Class rdf:about="techLayer4#Entity">
        <rdfs:label>Entity</rdfs:label>
        <rdfs:comment>Someone or something that is known to exist.</rdfs:comment>
        <rdfs:isDefinedBy rdf:resource="https://glossary.trustoverip.org/#term:entity"/>
    </owl:Class>

    <owl:Class rdf:about="techLayer4#TrustCommunity">
        <rdfs:label>Trust community</rdfs:label>
        <rdfs:comment>A set of parties who collaborate to achieve a mutual set of trust objectives.</rdfs:comment>
        <rdfs:isDefinedBy rdf:resource="https://glossary.trustoverip.org/#term:trust-community"/>
    </owl:Class>

    <owl:Class rdf:about="techLayer1#Identifier">
        <rdfs:label>Identifier</rdfs:label>
        <rdfs:comment>A single attribute—typically a character string—that uniquely identifies an entity within a specific context (which may be a global context). Examples include the name of a party, the URL of an organization, or a serial number for a man-made thing.</rdfs:comment>
        <rdfs:subClassOf rdf:resource="techLayer1#DigitalTrustUtility"/>
        <rdfs:isDefinedBy rdf:resource="https://glossary.trustoverip.org/#term:identifier"/>
    </owl:Class>

    <owl:Class rdf:about="techLayer1#Registry">
        <rdfs:label>Registry</rdfs:label>
        <rdfs:comment>A specialized database of records that serves as an authoritative source of information about entities.</rdfs:comment>
        <rdfs:subClassOf rdf:resource="techLayer1#DigitalTrustUtility"/>
        <rdfs:isDefinedBy rdf:resource="https://glossary.trustoverip.org/#term:registry"/>
    </owl:Class>



    <!-- ******************************* -->
    <!-- ********* Instance ************ -->
    <!-- ******************************* -->




</rdf:RDF>
