<rdf:RDF xmlns="http://example.org/techLayer1#"
    xml:base="http://example.org/techLayer1"
    xmlns:rdf="http://www.w3.org/1999/02/22-rdf-syntax-ns#"
    xmlns:owl="http://www.w3.org/2002/07/owl#"
    xmlns:rdfs="http://www.w3.org/2000/01/rdf-schema#"
    xmlns:xsd="http://www.w3.org/2001/XMLSchema#"
    xmlns:techLayer1="http://example.org/techLayer1#"
    xmlns:ex="http://example.org/someOtherNamespace#">


    <!-- ********************************************************************************************* -->
    <!-- *******************  All rights reserved to Cristian Lepore ********************************* -->
    <!-- ************************* Tech layer 1 of the ToIP model ************************************ -->
    <!-- ******** Definitions comes from the ToIP Glossary: https://glossary.trustoverip.org/ ******** -->
    <!-- ********************************************************************************************* -->

    <owl:Ontology rdf:about="http://example.org/techLayer1#">
        <rdfs:comment>Ontology representing the tech Layer 1 of the ToIP stack.</rdfs:comment>
    </owl:Ontology>





     <!-- ******************************* -->
     <!-- ********* Attribute *********** -->
     <!-- ******************************* -->




     <!-- ******************************* -->
     <!-- ********* Relation ************ -->
     <!-- ******************************* -->



     <!-- ******************************* -->
     <!-- * Connection with other Layer * -->
     <!-- ******************************* -->


     <owl:NamedIndividual rdf:about="techLayer1#URL">
          <rdf:type rdf:resource="techLayer1#Identifier"/>
          <rdfs:label>URL</rdfs:label>
          <identifiesEntity rdf:resource="techLayer1#Server"/>
          <identifiesEntity rdf:resource="techLayer1#issuerCA"/>
          <identifiesEntity rdf:resource="techLayer1#RootAuthority"/>
          <identifiesEntity rdf:resource="techLayer1#CA"/>
     </owl:NamedIndividual>





     <!-- ******************************* -->
     <!-- ********* Class *************** -->
     <!-- ******************************* -->

     <owl:Class rdf:about="techLayer1#TrustedCommunicationProtocol">
          <rdfs:label>Trusted Communication Protocol</rdfs:label>
          <rdfs:comment>The ToIP Trust Spanning Protocol (TSP) is the ToIP Layer 2 protocol for verifiable messaging that implements the trust spanning layer of the ToIP stack.  The TSP enables actors in different digital trust domains to interact in a similar way to how the Internet Protocol (IP) enables devices on different local area networks to exchange data.</rdfs:comment>
          <rdfs:isDefinedBy rdf:resource="https://glossary.trustoverip.org/#term:toip-trust-spanning-protocol"/>
     </owl:Class>


     <!-- ******************************* -->
     <!-- ********* Attribute *********** -->
     <!-- ******************************* -->

     <owl:DatatypeProperty rdf:about="techLayer1#edgeAgent">
          <rdfs:domain rdf:resource="techLayer1#UserAgent"/>
          <rdfs:range rdf:resource="http://www.w3.org/2001/XMLSchema#boolean"/>
          <rdfs:label>edge</rdfs:label>
          <rdfs:comment></rdfs:comment>
          <rdfs:isDefinedBy rdf:resource=""/>
     </owl:DatatypeProperty>




     <!-- ******************************* -->
     <!-- ********* Relation ************ -->
     <!-- ******************************* -->

      <owl:ObjectProperty rdf:about="techLayer1#implementsTrustTask">
            <rdfs:domain rdf:resource="techLayer1#TrustTaskProtocol"/>
            <rdfs:range rdf:resource="techLayer1#TrustTask"/>
            <rdfs:label>implements</rdfs:label>
            <rdfs:comment>A ToIP Layer 3 protocol that implements a specific trust task on behalf of a trust application operating at ToIP Layer 4.</rdfs:comment>
            <rdfs:isDefinedBy rdf:resource="https://glossary.trustoverip.org/#term:trust-task-protocol"/>
      </owl:ObjectProperty>

      <owl:ObjectProperty rdf:about="techLayer1#agencyOfUserAgent">
            <rdfs:domain rdf:resource="techLayer1#Actor"/>
            <rdfs:range rdf:resource="techLayer1#UserAgent"/>
            <rdfs:label>agency of</rdfs:label>
            <rdfs:comment>An entity that can act (do things/execute actions), e.g. people, machines, but not organizations. A digital agent can serve as an actor acting on behalf of its principal.</rdfs:comment>
            <rdfs:isDefinedBy rdf:resource="https://glossary.trustoverip.org/#term:actor"/>
      </owl:ObjectProperty>

      <owl:ObjectProperty rdf:about="techLayer1#issuanceCredential">
            <rdfs:domain rdf:resource="techLayer1#CredentialExchangeProtocol"/>
            <rdfs:range rdf:resource="techLayer1#Credential"/>
            <rdfs:label>issuance</rdfs:label>
            <rdfs:comment>The action of an issuer producing and transmitting a digital credential to a holder. A holder may request issuance by submitting an issuance request.</rdfs:comment>
            <rdfs:isDefinedBy rdf:resource="https://glossary.trustoverip.org/#term:issuance"/>
      </owl:ObjectProperty>

      <!-- Instance of protocol: CA -> server -->
      <owl:NamedIndividual rdf:about="techLayer1#ACME">
            <rdf:type rdf:resource="techLayer1#CredentialIssuanceProtocol"/>
            <rdfs:label>ACME</rdfs:label>
            <!-- Issuance credentials -->
            <techLayer1:issuanceCredential rdf:resource="techLayer1#X509CertificatePresentation"/>
            <techLayer1:issuanceCredential rdf:resource="techLayer1#X509CertificatePresentation2"/>
            <!-- Supports data format -->
            <techLayer1:supportsDataFormat rdf:resource="techLayer1#ASN1"/>
      </owl:NamedIndividual>

      <owl:NamedIndividual rdf:about="techLayer1#SCEP">
            <rdf:type rdf:resource="techLayer1#CredentialIssuanceProtocol"/>
            <rdfs:label>Simple Certificate Enrollment Protocol (SCEP)</rdfs:label>
            <!-- Issuance credentials -->
            <techLayer1:issuanceCredential rdf:resource="techLayer1#X509CertificatePresentation"/>

      <!-- Instance of the trust registry protocol -->
      <owl:NamedIndividual rdf:about="techLayer1#LDAP">
            <rdf:type rdf:resource="techLayer1#TrustRegistryProtocol"/>
            <rdfs:label>LDAP</rdfs:label>
      </owl:NamedIndividual>

      <owl:NamedIndividual rdf:about="techLayer1#HTTPTrustRegistryProtocol">
            <rdf:type rdf:resource="techLayer1#TrustRegistryProtocol"/>
            <rdfs:label>HTTP</rdfs:label>
      </owl:NamedIndividual>
      
      <owl:NamedIndividual rdf:about="techLayer1#WebsiteValidity">
            <rdf:type rdf:resource="techLayer1#TrustTask"/>
            <rdfs:label>Website validity</rdfs:label>
      </owl:NamedIndividual>






     <!-- ******************************* -->
     <!-- ********* Class *************** -->
     <!-- ******************************* -->

     <owl:Class rdf:about="techLayer1#TrustTask">
          <rdfs:label>Trust Task</rdfs:label>
          <rdfs:comment>A specific task that involves establishing, verifying, or maintaining trust relationships or exchanging verifiable messages or verifiable data that can be performed on behalf of a trust application by a trust task protocol at Layer 3 of the ToIP stack.</rdfs:comment>
          <rdfs:isDefinedBy rdf:resource="https://glossary.trustoverip.org/#term:trust-task"/>
     </owl:Class>
     
    <owl:Class rdf:about="techLayer1#Entity">
          <rdfs:label>Entity</rdfs:label>
          <rdfs:comment>Someone or something that is known to exist.</rdfs:comment>
          <rdfs:isDefinedBy rdf:resource="https://glossary.trustoverip.org/#term:entity"/>
    </owl:Class>



     <!-- ******************************* -->
     <!-- ********* Attribute *********** -->
     <!-- ******************************* -->

     <owl:DatatypeProperty rdf:about="techLayer1#includesConsent">
          <rdfs:domain rdf:resource="techLayer1#TrustTask"/>
          <rdfs:range rdf:resource="http://www.w3.org/2001/XMLSchema#boolean"/>
          <rdfs:label>includes consent</rdfs:label>
          <rdfs:comment>The data format extends the possibility to express consent data.</rdfs:comment>
     </owl:DatatypeProperty>



     <!-- ******************************* -->
     <!-- ********* Relation ************ -->
     <!-- ******************************* -->






    <!-- ******************************* -->
    <!-- ********* Class *************** -->
    <!-- ******************************* -->




    <!-- ******************************* -->
    <!-- ********* Relation ************ -->
    <!-- ******************************* -->

    <owl:ObjectProperty rdf:about="techLayer1#providesUserAgent">
        <rdfs:domain rdf:resource="techLayer1#TechnologyProvider"/>
        <rdfs:range rdf:resource="techLayer1#UserAgent"/>
        <rdfs:label>provides</rdfs:label>
        <rdfs:comment>The technology provider provides hardware and software for the user agent.</rdfs:comment>
    </owl:ObjectProperty>



    <!-- ******************************* -->
    <!-- ********* Attribute *********** -->
    <!-- ******************************* -->
     


    <!-- ******************************* -->
    <!-- * Connection with other Layer * -->
    <!-- ******************************* -->

    <owl:Class rdf:about="techLayer1#TechnologyProvider">
        <rdfs:label>Technology provider</rdfs:label>
        <rdfs:comment>Technology Providers are those things that implement the Technology Components. They are either Products (that you can buy, download, etc.) or they are configurations of other products in particular technical architectures, in which case they are called Technology Product Builds.</rdfs:comment>
        <rdfs:subClassOf rdf:resource="techLayer1#Organization"/>
        <rdfs:isDefinedBy rdf:resource="https://enterprise-architecture.org/university/defining-technology-providers/"/>
    </owl:Class>





    <!-- ******************************* -->
    <!-- ********* Class *************** -->
    <!-- ******************************* -->

    <owl:Class rdf:about="techLayer1#AuthoritativeSource">
        <rdfs:label>Authoritative source</rdfs:label>
        <rdfs:comment>A source of information that a relying party considers to be authoritative for that information. In ToIP architecture, the trust registry authorized by the governance framework for a trust community is typically considered an authoritative source by the members of that trust community. A system of record is an authoritative source for the data records it holds. A trust anchor is an authoritative source for the beginning of a trust chain.</rdfs:comment>
        <owl:equivalentClass rdf:resource="techLayer1#Registry"/>
        <rdfs:isDefinedBy rdf:resource="https://glossary.trustoverip.org/#term:authoritative-source"/>
    </owl:Class>

    <owl:Class rdf:about="techLayer1#Registrant">
        <rdfs:label>Registrant / Registration authority</rdfs:label>
        <rdfs:comment>The party submitting a registration record to a registry. Occasionally, it can be considered the Registration Authority in the PKI which verifies the identity of actors and approves requests.</rdfs:comment>
        <rdfs:subClassOf rdf:resource="techLayer1#AdministeringAuthority"/>
        <rdfs:isDefinedBy rdf:resource="https://glossary.trustoverip.org/#term:registrant"/>
    </owl:Class>



    <!-- ******************************* -->
    <!-- ********* Relation ************ -->
    <!-- ******************************* -->




    <!-- ******************************* -->
    <!-- ********* Attribute *********** -->
    <!-- ******************************* -->
     


    <!-- ******************************* -->
    <!-- * Connection with other Layer * -->
    <!-- ******************************* -->
    
    <owl:Class rdf:about="techLayer1#Holder">
        <rdfs:label>Holder</rdfs:label>
        <rdfs:comment>A role an agent performs by serving as the controller of the cryptographic keys and digital credentials in a digital wallet. The holder makes issuance requests for credentials and responds to presentation requests for credentials. A holder is usually, but not always, a subject of the credentials they are holding.</rdfs:comment>
        <rdfs:subClassOf rdf:resource="techLayer1#Actor"/>
        <rdfs:isDefinedBy rdf:resource="https://glossary.trustoverip.org/#term:holder"/>
    </owl:Class>

    <owl:Class rdf:about="techLayer1#TechnologyProvider">
        <rdfs:label>Technology provider</rdfs:label>
        <rdfs:comment>Technology Providers are those things that implement the Technology Components. They are either Products (that you can buy, download, etc.) or they are configurations of other products in particular technical architectures, in which case they are called Technology Product Builds.</rdfs:comment>
        <rdfs:subClassOf rdf:resource="techLayer1#Organization"/>
        <rdfs:isDefinedBy rdf:resource="https://enterprise-architecture.org/university/defining-technology-providers/"/>
    </owl:Class>


    <!-- ******************************* -->
    <!-- ********* Instance ************ -->
    <!-- ******************************* -->

    <!-- Instance of the registrant -->
    <owl:NamedIndividual rdf:about="techLayer1#RegistrationAuthority">
        <rdf:type rdf:resource="techLayer1#Registrant"/>
        <rdfs:label>Registration authority</rdfs:label>
        <!-- The Registration Authority registers the Server -->
        <techLayer1:registersHolder rdf:resource="techLayer1#Server"/>
    </owl:NamedIndividual>

    <!-- Instance of the repository -->
    <owl:NamedIndividual rdf:about="techLayer1#CRL">
        <rdf:type rdf:resource="techLayer1#AuthoritativeSource"/>
        <rdfs:label>Credential Revocation List (CRL)</rdfs:label>
    </owl:NamedIndividual>

    <owl:NamedIndividual rdf:about="techLayer1#CredentialRepository">
        <rdf:type rdf:resource="techLayer1#AuthoritativeSource"/>
        <rdfs:label>Credential repository</rdfs:label>
        <!-- Stores credentials -->
        <techLayer1:storesCredential rdf:resource="techLayer1#X509CertificatePresentation"/>
        <techLayer1:storesCredential rdf:resource="techLayer1#X509CertificatePresentation2"/>
    </owl:NamedIndividual>

    <owl:NamedIndividual rdf:about="techLayer1#ITU-T">
        <rdf:type rdf:resource="techLayer1#TechnologyProvider"/>
        <rdfs:label>ITU-T (International Telecommunication Union - Telecommunication Standardization Sector)</rdfs:label>
        <!-- Provides certificate standard -->
        <techLayer1:providesCredential rdf:resource="techLayer1#X509CertificatePresentation"/>
    </owl:NamedIndividual>






    <!-- ******************************* -->
    <!-- ********* Class *************** -->
    <!-- ******************************* -->


    <owl:ObjectProperty rdf:about="techLayer1#memberOfTrustCommunity">
        <rdfs:domain rdf:resource="techLayer1#Entity"/>
        <rdfs:range rdf:resource="techLayer1#TrustCommunity"/>
        <rdfs:label>member</rdfs:label>
    </owl:ObjectProperty>



    <!-- ******************************* -->
    <!-- ********* Attribute *********** -->
    <!-- ******************************* -->
     


    <!-- ******************************* -->
    <!-- * Connection with other Layer * -->
    <!-- ******************************* -->

    <owl:Class rdf:about="techLayer1#Organization">
        <rdfs:label>Organization</rdfs:label>
        <rdfs:comment>A party that consists of a group of parties who agree to be organized into a specific form in order to better achieve a common set of objectives. Examples include corporations, partnerships, sole proprietorships, non-profit organizations, associations, and governments.</rdfs:comment>
        <rdfs:subClassOf rdf:resource="techLayer1#Party"/>
        <rdfs:isDefinedBy rdf:resource="https://glossary.trustoverip.org/#term:organizations"/>
    </owl:Class>

    <owl:Class rdf:about="techLayer1#Party">
        <rdfs:label>Party</rdfs:label>
        <rdfs:comment>An entity that sets its objectives, maintains its knowledge, and uses that knowledge to pursue its objectives in an autonomous (sovereign) manner. Natural persons and organizations are the typical examples.</rdfs:comment>
        <rdfs:subClassOf rdf:resource="techLayer1#Entity"/>
        <rdfs:isDefinedBy rdf:resource="https://glossary.trustoverip.org/#term:party"/>
    </owl:Class>

     <owl:Class rdf:about="techLayer1#TrustCommunity">
          <rdfs:label>Trust community</rdfs:label>
          <rdfs:comment>A set of parties who collaborate to achieve a mutual set of trust objectives.</rdfs:comment>
          <rdfs:isDefinedBy rdf:resource="https://glossary.trustoverip.org/#term:trust-community"/>
     </owl:Class>



    <!-- ******************************* -->
    <!-- ********* Instance ************ -->
    <!-- ******************************* -->


    <!-- Instance of the accrediting authority -->
    <owl:NamedIndividual rdf:about="techLayer1#NationalAccreditor">
        <rdf:type rdf:resource="techLayer1#AccreditingAuthority"/>
        <rdfs:label>National accreditor</rdfs:label>
        <!-- accredits -->
        <techLayer1:accreditsAuditor rdf:resource="techLayer1#auditor"/>
    </owl:NamedIndividual>




</rdf:RDF>
