<?xml version="1.0"?>
<rdf:RDF xmlns="http://example.org/techLayer4#"
     xml:base="http://example.org/techLayer4"
     xmlns:rdf="http://www.w3.org/1999/02/22-rdf-syntax-ns#"
     xmlns:owl="http://www.w3.org/2002/07/owl#"
     xmlns:rdfs="http://www.w3.org/2000/01/rdf-schema#"
     xmlns:xsd="http://www.w3.org/2001/XMLSchema#">

     <!-- ********************************************************************************************* -->
     <!-- *******************  All rights reserved to Cristian Lepore ********************************* -->
     <!-- ************************* Tech layer 4 of the ToIP model ************************************ -->
     <!-- ******** Definitions comes from the ToIP Glossary: https://glossary.trustoverip.org/ ******** -->
     <!-- ********************************************************************************************* -->  
     
     <owl:Ontology rdf:about="http://example.org/techLayer4#">
          <rdfs:comment>Ontology representing the tech Layer 4 of the ToIP stack.</rdfs:comment>
     </owl:Ontology>



     <!-- ******************************* -->
     <!-- ********* Class *************** -->
     <!-- ******************************* -->

     <owl:Class rdf:about="techLayer4#TrustTask">
          <rdfs:label>Trust Task</rdfs:label>
          <rdfs:comment>A specific task that involves establishing, verifying, or maintaining trust relationships or exchanging verifiable messages or verifiable data that can be performed on behalf of a trust application by a trust task protocol at Layer 3 of the ToIP stack.</rdfs:comment>
          <rdfs:isDefinedBy rdf:resource="https://glossary.trustoverip.org/#term:trust-task"/>
     </owl:Class>

     <owl:Class rdf:about="techLayer4#Party">
          <rdfs:label>Party</rdfs:label>
          <rdfs:comment>An entity that sets its objectives, maintains its knowledge, and uses that knowledge to pursue its objectives in an autonomous (sovereign) manner. Natural persons and organizations are the typical examples.</rdfs:comment>
          <rdfs:subClassOf rdf:resource="techLayer4#Entity"/>
          <rdfs:isDefinedBy rdf:resource="https://glossary.trustoverip.org/#term:party"/>
     </owl:Class>



     <!-- ******************************* -->
     <!-- ********* Attribute *********** -->
     <!-- ******************************* -->




     <!-- ******************************* -->
     <!-- ********* Relation ************ -->
     <!-- ******************************* -->

     <owl:ObjectProperty rdf:about="techLayer4#actsOnBehalfOfPrincipal">
          <rdfs:domain rdf:resource="techLayer3#Actor"/>
          <rdfs:range rdf:resource="techLayer4#Principal"/>
          <rdfs:label>acts on behalf</rdfs:label>
          <rdfs:comment>The party for whom, or on behalf of whom, an actor is executing an action (this actor is then called an agent of that party).</rdfs:comment>
          <rdfs:isDefinedBy rdf:resource="https://glossary.trustoverip.org/#term:principal"/>
     </owl:ObjectProperty>




     <!-- ******************************* -->
     <!-- ******** Constraints ********** -->
     <!-- ******************************* -->

     <!-- Issuer, holder, verifier are disjoint -->
     <owl:AllDisjointClasses>
          <owl:members rdf:parseType="Collection">
               <rdf:Description rdf:about="techLayer3#Actor"/>
               <rdf:Description rdf:about="techLayer4#Organization"/>
          </owl:members>
     </owl:AllDisjointClasses>



     <!-- ******************************* -->
     <!-- * Connection with other Layer * -->
     <!-- ******************************* -->





     <!-- ******************************* -->
     <!-- ********* Instance ************ -->
     <!-- ******************************* -->



</rdf:RDF>
