<?xml version="1.0"?>
<rdf:RDF xmlns="http://example.org/techLayer4#"
     xml:base="http://example.org/techLayer4"
     xmlns:rdf="http://www.w3.org/1999/02/22-rdf-syntax-ns#"
     xmlns:owl="http://www.w3.org/2002/07/owl#"
     xmlns:rdfs="http://www.w3.org/2000/01/rdf-schema#"
     xmlns:xsd="http://www.w3.org/2001/XMLSchema#">

     <!-- ********************************************************************************************* -->
     <!-- *******************  All rights reserved to Cristian Lepore ********************************* -->
     <!-- ************************* Tech layer 4 of the ToIP model ************************************ -->
     <!-- ******** Definitions comes from the ToIP Glossary: https://glossary.trustoverip.org/ ******** -->
     <!-- ********************************************************************************************* -->  
     
     <owl:Ontology rdf:about="http://example.org/techLayer4#">
          <rdfs:comment>Ontology representing the tech Layer 4 of the ToIP stack.</rdfs:comment>
     </owl:Ontology>



     <!-- ******************************* -->
     <!-- ********* Class *************** -->
     <!-- ******************************* -->

     <owl:Class rdf:about="techLayer4#TrustTask">
          <rdfs:label>Trust Task</rdfs:label>
          <rdfs:comment>A specific task that involves establishing, verifying, or maintaining trust relationships or exchanging verifiable messages or verifiable data that can be performed on behalf of a trust application by a trust task protocol at Layer 3 of the ToIP stack.</rdfs:comment>
          <rdfs:isDefinedBy rdf:resource="https://glossary.trustoverip.org/#term:trust-task"/>
     </owl:Class>
     
     <owl:Class rdf:about="techLayer4#TrustApplication">
          <rdfs:label>Trust application</rdfs:label>
          <rdfs:comment>An application that runs at ToIP Layer 4 in order to perform trust tasks or engage in other verifiable messaging using the ToIP stack.</rdfs:comment>
          <rdfs:isDefinedBy rdf:resource="https://glossary.trustoverip.org/#term:trust-application"/>
     </owl:Class>

     <owl:Class rdf:about="techLayer4#Organization">
          <rdfs:label>Organization</rdfs:label>
          <rdfs:comment>A party that consists of a group of parties who agree to be organized into a specific form in order to better achieve a common set of objectives. Examples include corporations, partnerships, sole proprietorships, non-profit organizations, associations, and governments.</rdfs:comment>
          <rdfs:subClassOf rdf:resource="techLayer4#Party"/>
          <rdfs:isDefinedBy rdf:resource="https://glossary.trustoverip.org/#term:organizations"/>
     </owl:Class>

     <owl:Class rdf:about="techLayer4#TrustCommunity">
          <rdfs:label>Trust community</rdfs:label>
          <rdfs:comment>A set of parties who collaborate to achieve a mutual set of trust objectives.</rdfs:comment>
          <rdfs:isDefinedBy rdf:resource="https://glossary.trustoverip.org/#term:trust-community"/>
     </owl:Class>

     <owl:Class rdf:about="techLayer4#Principal">
          <rdfs:label>Principal</rdfs:label>
          <rdfs:comment>The party for whom, or on behalf of whom, an actor is executing an action (this actor is then called an agent of that party).</rdfs:comment>
          <rdfs:subClassOf rdf:resource="techLayer4#Party"/>
          <rdfs:isDefinedBy rdf:resource="https://glossary.trustoverip.org/#term:principal"/>
     </owl:Class>

     <owl:Class rdf:about="techLayer4#Party">
          <rdfs:label>Party</rdfs:label>
          <rdfs:comment>An entity that sets its objectives, maintains its knowledge, and uses that knowledge to pursue its objectives in an autonomous (sovereign) manner. Natural persons and organizations are the typical examples.</rdfs:comment>
          <rdfs:subClassOf rdf:resource="techLayer4#Entity"/>
          <rdfs:isDefinedBy rdf:resource="https://glossary.trustoverip.org/#term:party"/>
     </owl:Class>

    <owl:Class rdf:about="techLayer4#Entity">
          <rdfs:label>Entity</rdfs:label>
          <rdfs:comment>Someone or something that is known to exist.</rdfs:comment>
          <rdfs:isDefinedBy rdf:resource="https://glossary.trustoverip.org/#term:entity"/>
    </owl:Class>



     <!-- ******************************* -->
     <!-- ********* Attribute *********** -->
     <!-- ******************************* -->

     <owl:DatatypeProperty rdf:about="techLayer4#interim">
          <rdfs:domain rdf:resource="techLayer3#Actor"/>
          <rdfs:range rdf:resource="http://www.w3.org/2001/XMLSchema#dateTime"/>
          <rdfs:label>interim</rdfs:label>
          <rdfs:comment>Indicates the expiration date of the delegation.</rdfs:comment>
     </owl:DatatypeProperty>

     <owl:DatatypeProperty rdf:about="techLayer4#includesConsent">
          <rdfs:domain rdf:resource="techLayer4#TrustTask"/>
          <rdfs:range rdf:resource="http://www.w3.org/2001/XMLSchema#boolean"/>
          <rdfs:label>includes consent</rdfs:label>
          <rdfs:comment>The data format extends the possibility to express consent data.</rdfs:comment>
     </owl:DatatypeProperty>



     <!-- ******************************* -->
     <!-- ********* Relation ************ -->
     <!-- ******************************* -->

     <owl:ObjectProperty rdf:about="techLayer4#actsOnBehalfOfPrincipal">
          <rdfs:domain rdf:resource="techLayer3#Actor"/>
          <rdfs:range rdf:resource="techLayer4#Principal"/>
          <rdfs:label>acts on behalf</rdfs:label>
          <rdfs:comment>The party for whom, or on behalf of whom, an actor is executing an action (this actor is then called an agent of that party).</rdfs:comment>
          <rdfs:isDefinedBy rdf:resource="https://glossary.trustoverip.org/#term:principal"/>
     </owl:ObjectProperty>

     <owl:ObjectProperty rdf:about="techLayer4#memberOfTrustCommunity">
          <rdfs:domain rdf:resource="techLayer4#Entity"/>
          <rdfs:range rdf:resource="techLayer4#TrustCommunity"/>
          <rdfs:label>member</rdfs:label>
     </owl:ObjectProperty>

     <owl:ObjectProperty rdf:about="techLayer4#principalRepresentsOrganization">
          <rdfs:domain rdf:resource="techLayer4#Principal"/>
          <rdfs:range rdf:resource="techLayer4#Organization"/>
          <rdfs:label>represents</rdfs:label>
          <rdfs:comment>The principal may represent an organization.</rdfs:comment>
     </owl:ObjectProperty>

     <owl:ObjectProperty rdf:about="techLayer4#actorRepresentsOrganization">
          <rdfs:domain rdf:resource="techLayer3#Actor"/>
          <rdfs:range rdf:resource="techLayer4#Organization"/>
          <rdfs:label>represents</rdfs:label>
          <rdfs:comment>The actor may represent an organization.</rdfs:comment>
     </owl:ObjectProperty>

     <owl:ObjectProperty rdf:about="techLayer4#executesTrustApplication">
          <rdfs:domain rdf:resource="techLayer4#Party"/>
          <rdfs:range rdf:resource="techLayer4#TrustApplication"/>
          <rdfs:label>executes</rdfs:label>
          <rdfs:comment>An application that runs at ToIP Layer 4 in order to perform trust tasks or engage in other verifiable messaging using the ToIP stack.</rdfs:comment>
          <rdfs:isDefinedBy rdf:resource="https://glossary.trustoverip.org/#term:trust-application"/>
     </owl:ObjectProperty>

     <owl:ObjectProperty rdf:about="techLayer4#performsTrustTask">
          <rdfs:domain rdf:resource="techLayer4#TrustApplication"/>
          <rdfs:range rdf:resource="techLayer4#TrustTask"/>
          <rdfs:label>performs</rdfs:label>
          <rdfs:comment>An application that runs at ToIP Layer 4 in order to perform trust tasks or engage in other verifiable messaging using the ToIP stack.</rdfs:comment>
          <rdfs:isDefinedBy rdf:resource="https://glossary.trustoverip.org/#term:trust-application"/>
     </owl:ObjectProperty>



     <!-- ******************************* -->
     <!-- ******** Constraints ********** -->
     <!-- ******************************* -->

     <!-- Issuer, holder, verifier are disjoint -->
     <owl:AllDisjointClasses>
          <owl:members rdf:parseType="Collection">
               <rdf:Description rdf:about="techLayer3#Actor"/>
               <rdf:Description rdf:about="techLayer4#Organization"/>
          </owl:members>
     </owl:AllDisjointClasses>



     <!-- ******************************* -->
     <!-- * Connection with other Layer * -->
     <!-- ******************************* -->

     <owl:Class rdf:about="techLayer3#Actor">
          <rdfs:label>Actor</rdfs:label>
          <rdfs:comment>An entity that can act (do things/execute actions), e.g. people, machines, but not organizations. A digital agent can serve as an actor acting on behalf of its principal.</rdfs:comment>
          <rdfs:subClassOf rdf:resource="techLayer4#Party"/>
          <rdfs:isDefinedBy rdf:resource="https://glossary.trustoverip.org/#term:actor"/>
     </owl:Class>



     <!-- ******************************* -->
     <!-- ********* Instance ************ -->
     <!-- ******************************* -->



</rdf:RDF>
