<rdf:RDF xmlns="http://example.org/techLayer1#"
    xml:base="http://example.org/techLayer1"
    xmlns:rdf="http://www.w3.org/1999/02/22-rdf-syntax-ns#"
    xmlns:owl="http://www.w3.org/2002/07/owl#"
    xmlns:rdfs="http://www.w3.org/2000/01/rdf-schema#"
    xmlns:xsd="http://www.w3.org/2001/XMLSchema#"
    xmlns:techLayer1="http://example.org/techLayer1#"
    xmlns:ex="http://example.org/someOtherNamespace#">


    <!-- ********************************************************************************************* -->
    <!-- *******************  All rights reserved to Cristian Lepore ********************************* -->
    <!-- ************************* Tech layer 1 of the ToIP model ************************************ -->
    <!-- ********************************************************************************************* -->

    <owl:Ontology rdf:about="http://example.org/techLayer1#">
        <rdfs:comment>Ontology representing the tech Layer 1 of the ToIP stack.</rdfs:comment>
    </owl:Ontology>



     <!-- ******************************* -->
     <!-- ********* Class *************** -->
     <!-- ******************************* -->

     <owl:Class rdf:about="techLayer1#DigitalTrustUtility">
          <rdfs:label>Digital trust utility</rdfs:label>
          <rdfs:comment>An information system, network, distributed database, or blockchain designed to provide one or more supporting services to higher level components of decentralized digital trust infrastructure. In the ToIP stack, digital trust utilities are at Layer 1. A verifiable data registry is one type of digital trust utility.</rdfs:comment>
          <rdfs:isDefinedBy rdf:resource="https://glossary.trustoverip.org/#term:digital-trust-utility"/>
     </owl:Class>


     <owl:Class rdf:about="techLayer1#ArchitectureType">
          <rdfs:label>Architecture type</rdfs:label>
          <rdfs:comment>The type of architecture of a registry.</rdfs:comment>
          <rdfs:isDefinedBy rdf:resource="https://trustoverip.org/permalink/ToIP-Technical-Architecture-Specification-V1.0-PR1-2022-11-14.pdf"/>
     </owl:Class>

     <owl:Class rdf:about="techLayer1#CentralizedArchitecture">
          <rdfs:label>Centralized architecture</rdfs:label>
          <rdfs:comment>A centralized architecture of a registry.</rdfs:comment>
          <rdfs:subClassOf rdf:resource="techLayer1#ArchitectureType"/>
     </owl:Class>

     <owl:Class rdf:about="techLayer1#CentralizedIdentifier">
          <rdfs:label>Centralized identifier</rdfs:label>
          <rdfs:comment>A VID that requires a centralized registry.</rdfs:comment>
          <rdfs:subClassOf rdf:resource="techLayer1#VID"/>
          <rdfs:isDefinedBy rdf:resource="https://trustoverip.org/permalink/ToIP-Technical-Architecture-Specification-V1.0-PR1-2022-11-14.pdf"/>
     </owl:Class>




     <!-- ******************************* -->
     <!-- ********* Attribute *********** -->
     <!-- ******************************* -->

     <owl:DatatypeProperty rdf:about="techLayer1#permissioned">
          <rdfs:domain rdf:resource="techLayer1#Registry"/>
          <rdfs:range rdf:resource="http://www.w3.org/2001/XMLSchema#boolean"/>
          <rdfs:label>permissioned</rdfs:label>
          <rdfs:comment></rdfs:comment>
     </owl:DatatypeProperty>


     <!-- ******************************* -->
     <!-- ********* Relation ************ -->
     <!-- ******************************* -->

     <owl:ObjectProperty rdf:about="techLayer1#hasArchitectureType">
          <rdfs:domain rdf:resource="techLayer1#Registry"/>
          <rdfs:range rdf:resource="techLayer1#ArchitectureType"/>
          <rdfs:label>has</rdfs:label>
          <rdfs:comment>Specifies the type of architecture used by a registry (centralized, decentralized, federated).</rdfs:comment>
          <rdfs:isDefinedBy rdf:resource="https://trustoverip.org/permalink/ToIP-Technical-Architecture-Specification-V1.0-PR1-2022-11-14.pdf"/>
     </owl:ObjectProperty>

     <owl:ObjectProperty rdf:about="techLayer1#storesMetadata">
          <rdfs:domain rdf:resource="techLayer1#VDR"/>
          <rdfs:range rdf:resource="techLayer1#Metadata"/>
          <rdfs:label>stores</rdfs:label>
          <rdfs:comment>A registry that facilitates the creation, verification, updating, and/or deactivation of decentralized identifiers and DID documents. A verifiable data registry may also be used for other cryptographically-verifiable data structures such as verifiable credentials.</rdfs:comment>
          <rdfs:isDefinedBy rdf:resource="https://glossary.trustoverip.org/#term:registry"/>
     </owl:ObjectProperty>

     <owl:ObjectProperty rdf:about="techLayer1#resolvesRegistry">
          <rdfs:domain rdf:resource="techLayer1#Registry"/>
          <rdfs:range rdf:resource="techLayer1#Registry"/>
          <rdfs:label>resolves</rdfs:label>
          <rdfs:comment>A (meta)registry points to other (meta)registries for interoperability across systems.</rdfs:comment>
          <rdfs:isDefinedBy rdf:resource="http://ayra.forum/wp-content/uploads/2025/01/Ayra-Technical-Whitepaper-v0.0.10.pdf"/>
     </owl:ObjectProperty>



     <!-- ******************************* -->
     <!-- * Connection with other Layer * -->
     <!-- ******************************* -->

     <owl:Class rdf:about="techLayer1#Entity">
          <rdfs:label>Entity</rdfs:label>
          <rdfs:comment>Someone or something that is known to exist.</rdfs:comment>
          <rdfs:isDefinedBy rdf:resource="https://glossary.trustoverip.org/#term:entity"/>
     </owl:Class>

     <owl:ObjectProperty rdf:about="techLayer1#issuerRegisteredInRegistry">
          <rdfs:domain rdf:resource="techLayer1#Issuer"/>
          <rdfs:range rdf:resource="techLayer1#Registry"/>
          <rdfs:label>registered in</rdfs:label>
          <rdfs:comment>The issuer is registered in the registry.</rdfs:comment>
          <rdfs:isDefinedBy rdf:resource="http://ayra.forum/wp-content/uploads/2025/01/Ayra-Technical-Whitepaper-v0.0.10.pdf"/>
     </owl:ObjectProperty>

     <owl:ObjectProperty rdf:about="techLayer1#verifierRegisteredInRegistry">
          <rdfs:domain rdf:resource="techLayer1#Verifier"/>
          <rdfs:range rdf:resource="techLayer1#Registry"/>
          <rdfs:label>registered in</rdfs:label>
          <rdfs:comment>The verifier is registered in the registry.</rdfs:comment>
          <rdfs:isDefinedBy rdf:resource="http://ayra.forum/wp-content/uploads/2025/01/Ayra-Technical-Whitepaper-v0.0.10.pdf"/>
     </owl:ObjectProperty>



     <!-- ******************************* -->
     <!-- ********* Instance ************ -->
     <!-- ******************************* -->

     <owl:NamedIndividual rdf:about="techLayer1#RelyingPartyIdentifier">
          <rdf:type rdf:resource="techLayer1#CentralizedIdentifier"/>
          <rdfs:label>Relying Party Identifier</rdfs:label>
          <techLayer1:reliesOnCentralizedRegistry rdf:resource="techLayer1#centralizedArchitecture"/>
          <techLayer1:identifiesEntity rdf:resource="techLayer1#RelyingParty"/>
     </owl:NamedIndividual>

     <owl:NamedIndividual rdf:about="techLayer1#AttestationProviderIdentifier">
          <rdf:type rdf:resource="techLayer1#CentralizedIdentifier"/>
          <rdfs:label>Attestation Provider Identifier</rdfs:label>
          <techLayer1:reliesOnCentralizedRegistry rdf:resource="techLayer1#centralizedArchitecture"/>
          <techLayer1:identifiesEntity rdf:resource="techLayer1#QEAAIssuer"/>
          <techLayer1:identifiesEntity rdf:resource="techLayer1#PuB-EAAIssuer"/>
          <techLayer1:identifiesEntity rdf:resource="techLayer1#EAAIssuer"/>
          <techLayer1:identifiesEntity rdf:resource="techLayer1#QESRCIssuer"/>
     </owl:NamedIndividual>

     <owl:NamedIndividual rdf:about="techLayer1#TrustedListPIDProviders">
          <rdf:type rdf:resource="techLayer1#VDR"/>
          <rdfs:label>Trusted List of PID Providers</rdfs:label>
          <techLayer1:hasArchitectureType rdf:resource="techLayer1#centralizedArchitecture"/>
          <techLayer1:storesMetadata rdf:resource="techLayer1#TrustAnchor"/>
          <techLayer1:maintainsIdentifier rdf:resource="techLayer1#PubKey"/>
          <techLayer1:maintainsIdentifier rdf:resource="techLayer1#EUIdentifier"/>
          <techLayer1:maintainsIdentifier rdf:resource="techLayer1#PIDProviderIdentifier"/>
          <!-- Public: true -->
          <techLayer1:public rdf:datatype="http://www.w3.org/2001/XMLSchema#boolean">true</techLayer1:public>
          <!-- Permissioned: true -->
          <techLayer1:permissioned rdf:datatype="http://www.w3.org/2001/XMLSchema#boolean">true</techLayer1:permissioned>
     </owl:NamedIndividual>

      <!-- ******************************* -->
      <!-- ******** Constraints ********** -->
      <!-- ******************************* -->

      <!-- Issuer, holder, verifier are disjoint -->
      <owl:AllDisjointClasses>
            <owl:members rdf:parseType="Collection">
                  <rdf:Description rdf:about="techLayer1#Issuer"/>
                  <rdf:Description rdf:about="techLayer1#Holder"/>
                  <rdf:Description rdf:about="techLayer1#Verifier"/>
            </owl:members>
      </owl:AllDisjointClasses>



      <!-- ******************************* -->
      <!-- * Connection with other Layer * -->
      <!-- ******************************* -->


      <!-- Instance of holder -->
      <owl:NamedIndividual rdf:about="techLayer1#holder">
            <rdf:type rdf:resource="techLayer1#Holder"/>
            <rdfs:label>Holder</rdfs:label>
            <techLayer1:agencyOfUserAgent rdf:resource="techLayer1#EUDIWallet"/>
            <techLayer1:agencyOfUserAgent rdf:resource="techLayer1#EUDIWallet2"/>
            <techLayer1:usesTrustTaskProtocol rdf:resource="techLayer1#HTTPTrustRegistryProtocol"/>
            <techLayer1:usesTrustTaskProtocol rdf:resource="techLayer1#LDAP"/>
            <techLayer1:usesTrustTaskProtocol rdf:resource="techLayer1#OIDC4VP"/>
            <techLayer1:usesTrustTaskProtocol rdf:resource="techLayer1#ISO18013-5Protocol"/>
            <techLayer1:actsOnBehalfOfPrincipal rdf:resource="techLayer1#Citizen"/>
            <techLayer1:holderConsultsAuthoritativeSource rdf:resource="techLayer1#RPRegistry"/>
            <techLayer1:holderConsultsAuthoritativeSource rdf:resource="techLayer1#QTSPRegistry"/>
            <techLayer1:holderConsultsAuthoritativeSource rdf:resource="techLayer1#ACLRegistry"/>
            <techLayer1:holderConsultsAuthoritativeSource rdf:resource="techLayer1#RPIntermediaryRegistry"/>
            <techLayer1:holderConsultsAuthoritativeSource rdf:resource="techLayer1#WalletElementList"/>
      </owl:NamedIndividual>

      <!-- Instance of verifier -->
      <owl:NamedIndividual rdf:about="techLayer1#RelyingParty">
            <rdf:type rdf:resource="techLayer1#Verifier"/>
            <rdfs:label>Relying Party</rdfs:label>
            <techLayer1:usesTrustTaskProtocol rdf:resource="techLayer1#HTTPTrustRegistryProtocol"/>
            <techLayer1:usesTrustTaskProtocol rdf:resource="techLayer1#LDAP"/>
            <techLayer1:actorRepresentsOrganization rdf:resource="techLayer1#IRIT"/>
            <techLayer1:verifierConsultsAuthoritativeSource rdf:resource="techLayer1#QTSPRegistry"/>
      </owl:NamedIndividual>

      <owl:NamedIndividual rdf:about="techLayer1#Title">
            <rdf:type rdf:resource="techLayer1#Attribute"/>
            <rdfs:label>Place of Birth</rdfs:label>
      </owl:NamedIndividual>

      <!-- Instance of the trust registry protocol -->
      <owl:NamedIndividual rdf:about="techLayer1#LDAP">
            <rdf:type rdf:resource="techLayer1#TrustRegistryProtocol"/>
            <rdfs:label>LDAP</rdfs:label>
            <techLayer1:consultsRegistry rdf:resource="techLayer1#TrustedListWalletProviders"/>
            <techLayer1:consultsRegistry rdf:resource="techLayer1#TrustedListPIDProviders"/>
            <techLayer1:consultsRegistry rdf:resource="techLayer1#TrustedListQEAAProviders"/>
            <techLayer1:consultsRegistry rdf:resource="techLayer1#TrustedListPuB-EAAProviders"/>
            <techLayer1:consultsRegistry rdf:resource="techLayer1#TrustedListQESRCProviders"/>
            <techLayer1:consultsRegistry rdf:resource="techLayer1#TrustedListACA"/>
            <techLayer1:consultsRegistry rdf:resource="techLayer1#TrustedListACA2"/>
      </owl:NamedIndividual>


    <owl:NamedIndividual rdf:about="techLayer1#MemberState">
        <rdf:type rdf:resource="techLayer1#AdministeringAuthority"/>
        <rdfs:label>Member State</rdfs:label>
        <techLayer1:administersDigitalTrustUtility rdf:resource="techLayer1#TrustedListWalletProviders"/>
        <techLayer1:administersDigitalTrustUtility rdf:resource="techLayer1#TrustedListPIDProviders"/>
        <techLayer1:administersDigitalTrustUtility rdf:resource="techLayer1#TrustedListQEAAProviders"/>
        <techLayer1:administersDigitalTrustUtility rdf:resource="techLayer1#TrustedListPuB-EAAProviders"/>
        <techLayer1:administersDigitalTrustUtility rdf:resource="techLayer1#TrustedListQESRCProviders"/>
        <techLayer1:administersDigitalTrustUtility rdf:resource="techLayer1#TrustedListACA"/>
        <techLayer1:administersDigitalTrustUtility rdf:resource="techLayer1#TrustedListACA2"/>
    </owl:NamedIndividual>




    <!-- ******************************* -->
    <!-- * Connection with other Layer * -->
    <!-- ******************************* -->

    <owl:ObjectProperty rdf:about="techLayer1#enforcesGovernanceFramework">
        <rdfs:domain rdf:resource="techLayer1#GoverningAuthority"/>
        <rdfs:range rdf:resource="techLayer1#GovernanceFramework"/>
        <rdfs:label>enforces</rdfs:label>
        <rdfs:comment>The party (or set of parties) authoritative for governing a trust community, usually (but not always) by developing, publishing, maintaining, and enforcing a governance framework. A governing body may be a government, a formal legal entity of any kind, an informal group of any kind, or an individual. A governing body may also delegate operational responsibilities to an administering body.</rdfs:comment>
        <rdfs:isDefinedBy rdf:resource="https://glossary.trustoverip.org/#term:governing-authority"/>
    </owl:ObjectProperty>



    <!-- ******************************* -->
    <!-- ********* Attribute *********** -->
    <!-- ******************************* -->
     
    <owl:DatatypeProperty rdf:about="techLayer1#open">
        <rdfs:domain rdf:resource="techLayer1#TechnicalStandard"/>
        <rdfs:range rdf:resource="http://www.w3.org/2001/XMLSchema#boolean"/>
        <rdfs:label>open</rdfs:label>
        <rdfs:comment>Indicates whether the technical standards are open to public review and comment.</rdfs:comment>
    </owl:DatatypeProperty>



    <!-- ******************************* -->
    <!-- * Connection with other Layer * -->
    <!-- ******************************* -->

    <owl:Class rdf:about="techLayer1#TechnologyProvider">
        <rdfs:label>Technology provider</rdfs:label>
        <rdfs:comment>Technology Providers are those things that implement the Technology Components. They are either Products (that you can buy, download, etc.) or they are configurations of other products in particular technical architectures, in which case they are called Technology Product Builds.</rdfs:comment>
        <rdfs:subClassOf rdf:resource="techLayer1#Organization"/>
        <rdfs:isDefinedBy rdf:resource="https://enterprise-architecture.org/university/defining-technology-providers/"/>
    </owl:Class>

    <owl:ObjectProperty rdf:about="techLayer1#providesProof">
        <rdfs:domain rdf:resource="techLayer1#TechnologyProvider"/>
        <rdfs:range rdf:resource="techLayer1#Proof"/>
        <rdfs:label>provides</rdfs:label>
        <rdfs:comment>The technology provider provides hardware and software for the proofs.</rdfs:comment>
    </owl:ObjectProperty>



    <!-- ******************************* -->
    <!-- ********* Attribute *********** -->
    <!-- ******************************* -->

    <owl:DatatypeProperty rdf:about="techLayer1#open">
        <rdfs:domain rdf:resource="techLayer1#TechnicalStandard"/>
        <rdfs:range rdf:resource="http://www.w3.org/2001/XMLSchema#boolean"/>
        <rdfs:label>open</rdfs:label>
        <rdfs:comment>Indicates whether the technical standards are open to public review and comment.</rdfs:comment>
    </owl:DatatypeProperty>


    <!-- ******************************* -->
    <!-- * Connection with other Layer * -->
    <!-- ******************************* -->
    
    <owl:Class rdf:about="techLayer1#Holder">
        <rdfs:label>Holder</rdfs:label>
        <rdfs:comment>A role an agent performs by serving as the controller of the cryptographic keys and digital credentials in a digital wallet. The holder makes issuance requests for credentials and responds to presentation requests for credentials. A holder is usually, but not always, a subject of the credentials they are holding.</rdfs:comment>
        <rdfs:subClassOf rdf:resource="techLayer1#Actor"/>
        <rdfs:isDefinedBy rdf:resource="https://glossary.trustoverip.org/#term:holder"/>
    </owl:Class>


    <!-- ******************************* -->
    <!-- ********* Relation ************ -->
    <!-- ******************************* -->

    <owl:ObjectProperty rdf:about="techLayer1#leveragesRiskLevel">
        <rdfs:domain rdf:resource="techLayer1#Auditor"/>
        <rdfs:range rdf:resource="techLayer1#RiskLevel"/>
        <rdfs:label>leverages</rdfs:label>
        <rdfs:comment>Formal declaration by an accrediting authority that an information system is approved to operate at an acceptable level of risk, based on the implementation of an approved set of technical, managerial, and procedural safeguards.</rdfs:comment>
        <rdfs:isDefinedBy rdf:resource="https://glossary.trustoverip.org/#term:accreditation"/>
    </owl:ObjectProperty>

    <owl:ObjectProperty rdf:about="techLayer1#accreditsAuditor">
        <rdfs:domain rdf:resource="techLayer1#AccreditingAuthority"/>
        <rdfs:range rdf:resource="techLayer1#Auditor"/>
        <rdfs:label>accredits</rdfs:label>
        <rdfs:comment>Formal declaration by an accrediting authority that an information system is approved to operate at an acceptable level of risk, based on the implementation of an approved set of technical, managerial, and procedural safeguards.</rdfs:comment>
        <rdfs:isDefinedBy rdf:resource="https://glossary.trustoverip.org/#term:accreditation"/>
    </owl:ObjectProperty>

    <owl:ObjectProperty rdf:about="techLayer1#auditsEntity">
        <rdfs:domain rdf:resource="techLayer1#Auditor"/>
        <rdfs:range rdf:resource="techLayer1#Entity"/>
        <rdfs:label>audits</rdfs:label>
        <rdfs:comment>Independent review and examination of records and activities to assess the adequacy of system controls, to ensure compliance with established policies and operational procedures.</rdfs:comment>
        <rdfs:isDefinedBy rdf:resource="https://glossary.trustoverip.org/#term:audit"/>
    </owl:ObjectProperty>

    <owl:NamedIndividual rdf:about="techLayer1#RiskBasedApproach">
        <rdf:type rdf:resource="techLayer1#RiskLevel"/>
        <rdfs:label>Risk-Based Approach</rdfs:label>
    </owl:NamedIndividual>



</rdf:RDF>
