<?xml version="1.0"?>
<rdf:RDF xmlns="http://example.org/govLayer3#"
    xml:base="http://example.org/govLayer3"
    xmlns:rdf="http://www.w3.org/1999/02/22-rdf-syntax-ns#"
    xmlns:owl="http://www.w3.org/2002/07/owl#"
    xmlns:rdfs="http://www.w3.org/2000/01/rdf-schema#"
    xmlns:xsd="http://www.w3.org/2001/XMLSchema#">



    <!-- ********************************************************************************************* -->
    <!-- *******************  All rights reserved to Cristian Lepore ********************************* -->
    <!-- ************************* Gov layer 3 of the ToIP model ************************************* -->
    <!-- ******** Definitions comes from the ToIP Glossary: https://glossary.trustoverip.org/ ******** -->
    <!-- ********************************************************************************************* -->

    <owl:Ontology rdf:about="http://example.org/govLayer3#">
        <rdfs:comment>Ontology representing the governance Layer 3 of the ToIP stack.</rdfs:comment>
    </owl:Ontology>



    <!-- ******************************* -->
    <!-- ********* Class *************** -->
    <!-- ******************************* -->

    <owl:Class rdf:about="govLayer3#AuthoritativeSource">
        <rdfs:label>Authoritative source</rdfs:label>
        <rdfs:comment>A source of information that a relying party considers to be authoritative for that information. In ToIP architecture, the trust registry authorized by the governance framework for a trust community is typically considered an authoritative source by the members of that trust community. A system of record is an authoritative source for the data records it holds. A trust anchor is an authoritative source for the beginning of a trust chain.</rdfs:comment>
        <owl:equivalentClass rdf:resource="techLayer1#Registry"/>
        <owl:equivalentClass rdf:resource="techLayer1#TrustRegistry"/>
        <owl:equivalentClass rdf:resource="techLayer1#TrustList"/>
        <rdfs:isDefinedBy rdf:resource="https://glossary.trustoverip.org/#term:authoritative-source"/>
    </owl:Class>

    <owl:Class rdf:about="govLayer3#Registrant">
        <rdfs:label>Registrant / Registration authority</rdfs:label>
        <rdfs:comment>The party submitting a registration record to a registry. Occasionally, it can be considered the Registration Authority in the PKI which verifies the identity of actors and approves requests.</rdfs:comment>
        <rdfs:subClassOf rdf:resource="governance#AdministeringAuthority"/>
        <rdfs:isDefinedBy rdf:resource="https://glossary.trustoverip.org/#term:registrant"/>
    </owl:Class>

    <owl:Class rdf:about="govLayer3#Insurer">
        <rdfs:label>Insurer</rdfs:label>
        <rdfs:comment>A person or company that insures someone or something.</rdfs:comment>
        <rdfs:isDefinedBy rdf:resource="https://dictionary.cambridge.org/dictionary/english/insurer"/>
    </owl:Class>

    <owl:Class rdf:about="govLayer3#RiskLevel">
        <rdfs:label>Risk level</rdfs:label>
        <rdfs:comment></rdfs:comment>
    </owl:Class>



    <!-- ******************************* -->
    <!-- ********* Relation ************ -->
    <!-- ******************************* -->

    <owl:ObjectProperty rdf:about="govLayer3#adoptsTechnicalStandard">
        <rdfs:domain rdf:resource="govLayer1#TechnologyProvider"/>
        <rdfs:range rdf:resource="govLayer1#TechnicalStandard"/>
        <rdfs:label>adopts</rdfs:label>
        <rdfs:comment>The technology provider adopts technical standards.</rdfs:comment>
    </owl:ObjectProperty>

    <owl:ObjectProperty rdf:about="govLayer3#identifiesRiskLevel">
        <rdfs:domain rdf:resource="governance#ControlledDocument"/>
        <rdfs:range rdf:resource="govLayer3#RiskLevel"/>
        <rdfs:label>identifies</rdfs:label>
        <rdfs:comment>The process of identifying risks to organizational operations (including mission, functions, image, reputation), organizational assets, individuals, other organizations, and the overall ecosystem, resulting from the operation of an information system. Risk assessment is part of risk management, incorporates threat and vulnerability analyses, and considers risk mitigations provided by security controls planned or in place.</rdfs:comment>
        <rdfs:isDefinedBy rdf:resource="https://glossary.trustoverip.org/#term:risk-assessment"/>
    </owl:ObjectProperty>

    <owl:ObjectProperty rdf:about="govLayer3#storesCredential">
        <rdfs:domain rdf:resource="govLayer3#AuthoritativeSource"/>
        <rdfs:range rdf:resource="techLayer3#Credential"/>
        <rdfs:label>stores</rdfs:label>
        <rdfs:comment>A source of information that a relying party considers to be authoritative for that information. In ToIP architecture, the trust registry authorized by the governance framework for a trust community is typically considered an authoritative source by the members of that trust community. A system of record is an authoritative source for the data records it holds. A trust anchor is an authoritative source for the beginning of a trust chain.</rdfs:comment>
        <rdfs:isDefinedBy rdf:resource="https://glossary.trustoverip.org/#term:authoritative-source"/>
    </owl:ObjectProperty>

    <owl:ObjectProperty rdf:about="govLayer3#storesProof">
        <rdfs:domain rdf:resource="govLayer3#AuthoritativeSource"/>
        <rdfs:range rdf:resource="techLayer3#Proof"/>
        <rdfs:label>stores</rdfs:label>
        <rdfs:comment>A source of information that a relying party considers to be authoritative for that information. In ToIP architecture, the trust registry authorized by the governance framework for a trust community is typically considered an authoritative source by the members of that trust community. A system of record is an authoritative source for the data records it holds. A trust anchor is an authoritative source for the beginning of a trust chain.</rdfs:comment>
        <rdfs:isDefinedBy rdf:resource="https://glossary.trustoverip.org/#term:authoritative-source"/>
    </owl:ObjectProperty>

    <owl:ObjectProperty rdf:about="govLayer3#issuerConsultsAuthoritativeSource">
        <rdfs:domain rdf:resource="techLayer3#Issuer"/>
        <rdfs:range rdf:resource="govLayer3#AuthoritativeSource"/>
        <rdfs:label>consults</rdfs:label>
        <rdfs:comment>The issuer queries the authoritative source of information, for example to discover the credential schemes and attributes. Paper: Lepore, Cristian, Romain Laborde, and Jessica Eynard. Aligning eIDAS and Trust Over IP: A Mapping Approach. Proceedings of the 19th International Conference on Availability, Reliability and Security. 2024.</rdfs:comment>
        <rdfs:isDefinedBy rdf:resource="https://doi.org/10.1007/978-3-031-89350-6_4"/>
    </owl:ObjectProperty>

    <owl:ObjectProperty rdf:about="govLayer3#verifierConsultsAuthoritativeSource">
        <rdfs:domain rdf:resource="techLayer3#Verifier"/>
        <rdfs:range rdf:resource="govLayer3#AuthoritativeSource"/>
        <rdfs:label>consults</rdfs:label>
        <rdfs:comment>The verifier queries the authoritative source of information, for example to discover the credential schemes and attributes. Paper: Lepore, Cristian, Romain Laborde, and Jessica Eynard. Aligning eIDAS and Trust Over IP: A Mapping Approach. Proceedings of the 19th International Conference on Availability, Reliability and Security. 2024.</rdfs:comment>
        <rdfs:isDefinedBy rdf:resource="https://doi.org/10.1007/978-3-031-89350-6_4"/>
    </owl:ObjectProperty>

    <owl:ObjectProperty rdf:about="govLayer3#holderConsultsAuthoritativeSource">
        <rdfs:domain rdf:resource="techLayer3#Holder"/>
        <rdfs:range rdf:resource="govLayer3#AuthoritativeSource"/>
        <rdfs:label>consults</rdfs:label>
        <rdfs:comment>The holder queries the authoritative source of information, for example to discover the credential schemes and attributes. Paper: Lepore, Cristian, Romain Laborde, and Jessica Eynard. Aligning eIDAS and Trust Over IP: A Mapping Approach. Proceedings of the 19th International Conference on Availability, Reliability and Security. 2024.</rdfs:comment>
        <rdfs:isDefinedBy rdf:resource="https://doi.org/10.1007/978-3-031-89350-6_4"/>
    </owl:ObjectProperty>

    <owl:ObjectProperty rdf:about="govLayer3#registersIssuer">
        <rdfs:domain rdf:resource="govLayer3#Registrant"/>
        <rdfs:range rdf:resource="techLayer3#Issuer"/>
        <rdfs:label>registers</rdfs:label>
        <rdfs:comment>The party submitting a registration record to a registry.</rdfs:comment>
        <rdfs:isDefinedBy rdf:resource="https://glossary.trustoverip.org/#term:registrant"/>
    </owl:ObjectProperty>

    <owl:ObjectProperty rdf:about="govLayer3#registersHolder">
        <rdfs:domain rdf:resource="govLayer3#Registrant"/>
        <rdfs:range rdf:resource="techLayer3#Holder"/>
        <rdfs:label>registers</rdfs:label>
        <rdfs:comment>The party submitting a registration record to a registry.</rdfs:comment>
        <rdfs:isDefinedBy rdf:resource="https://glossary.trustoverip.org/#term:registrant"/>
    </owl:ObjectProperty>

    <owl:ObjectProperty rdf:about="govLayer3#registersVerifier">
        <rdfs:domain rdf:resource="govLayer3#Registrant"/>
        <rdfs:range rdf:resource="techLayer3#Verifier"/>
        <rdfs:label>registers</rdfs:label>
        <rdfs:comment>The party submitting a registration record to a registry.</rdfs:comment>
        <rdfs:isDefinedBy rdf:resource="https://glossary.trustoverip.org/#term:registrant"/>
    </owl:ObjectProperty>

    <owl:ObjectProperty rdf:about="govLayer3#executesControlledDocument">
        <rdfs:domain rdf:resource="govLayer3#Insurer"/>
        <rdfs:range rdf:resource="governance#ControlledDocument"/>
        <rdfs:label>executes</rdfs:label>
        <rdfs:comment>The insurer executes the risk assessment.</rdfs:comment>
    </owl:ObjectProperty>

    <owl:ObjectProperty rdf:about="govLayer3#providesTrustTaskProtocol">
        <rdfs:domain rdf:resource="govLayer1#TechnologyProvider"/>
        <rdfs:range rdf:resource="techLayer3#TrustTaskProtocol"/>
        <rdfs:label>provides</rdfs:label>
        <rdfs:comment>The technology provider provides hardware and software for the Trust Task Protocol.</rdfs:comment>
    </owl:ObjectProperty>

    <owl:ObjectProperty rdf:about="govLayer3#providesCredential">
        <rdfs:domain rdf:resource="govLayer1#TechnologyProvider"/>
        <rdfs:range rdf:resource="techLayer3#Credential"/>
        <rdfs:label>provides</rdfs:label>
        <rdfs:comment>The technology provider provides hardware and software for credentials.</rdfs:comment>
    </owl:ObjectProperty>

    <owl:ObjectProperty rdf:about="govLayer3#providesProof">
        <rdfs:domain rdf:resource="govLayer1#TechnologyProvider"/>
        <rdfs:range rdf:resource="techLayer3#Proof"/>
        <rdfs:label>provides</rdfs:label>
        <rdfs:comment>The technology provider provides hardware and software for the proofs.</rdfs:comment>
    </owl:ObjectProperty>



    <!-- ******************************* -->
    <!-- ********* Attribute *********** -->
    <!-- ******************************* -->

    <owl:DatatypeProperty rdf:about="govLayer1#open">
        <rdfs:domain rdf:resource="govLayer1#TechnicalStandard"/>
        <rdfs:range rdf:resource="http://www.w3.org/2001/XMLSchema#boolean"/>
        <rdfs:label>open</rdfs:label>
        <rdfs:comment>Indicates whether the technical standards are open to public review and comment.</rdfs:comment>
    </owl:DatatypeProperty>


    <!-- ******************************* -->
    <!-- * Connection with other Layer * -->
    <!-- ******************************* -->
    
    <owl:Class rdf:about="techLayer3#Holder">
        <rdfs:label>Holder</rdfs:label>
        <rdfs:comment>A role an agent performs by serving as the controller of the cryptographic keys and digital credentials in a digital wallet. The holder makes issuance requests for credentials and responds to presentation requests for credentials. A holder is usually, but not always, a subject of the credentials they are holding.</rdfs:comment>
        <rdfs:subClassOf rdf:resource="techLayer3#Actor"/>
        <rdfs:isDefinedBy rdf:resource="https://glossary.trustoverip.org/#term:holder"/>
    </owl:Class>

    <owl:Class rdf:about="governance#ControlledDocument">
        <rdfs:label>Controlled document</rdfs:label>
        <rdfs:comment>A governance document whose authority is derived from a primary document.</rdfs:comment>
        <rdfs:subClassOf rdf:resource="governance#GovernanceDocument"/>
        <rdfs:isDefinedBy rdf:resource="https://glossary.trustoverip.org/#term:controlled-document"/>
    </owl:Class>

    <owl:Class rdf:about="govLayer1#TechnologyProvider">
        <rdfs:label>Technology provider</rdfs:label>
        <rdfs:comment>Technology Providers are those things that implement the Technology Components. They are either Products (that you can buy, download, etc.) or they are configurations of other products in particular technical architectures, in which case they are called Technology Product Builds.</rdfs:comment>
        <rdfs:subClassOf rdf:resource="techLayer4#Organization"/>
        <rdfs:isDefinedBy rdf:resource="https://enterprise-architecture.org/university/defining-technology-providers/"/>
    </owl:Class>

    <owl:Class rdf:about="govLayer1#HardwareManufacturer">
        <rdfs:label>Hardware manufacturer</rdfs:label>
        <rdfs:comment>A business or company which makes goods in large quantities to sell.</rdfs:comment>
        <rdfs:subClassOf rdf:resource="govLayer1#TechnologyProvider"/>
        <rdfs:isDefinedBy rdf:resource="https://www.collinsdictionary.com/dictionary/english/hardware-manufacturer"/>
    </owl:Class>

    <owl:Class rdf:about="govLayer1#SoftwarePublisher">
        <rdfs:label>Software publisher</rdfs:label>
        <rdfs:comment>A software publisher is a publishing company in the software industry between the developer and the distributor. In some companies, two or all three of these roles may be combined (and indeed, may reside in a single person, especially in the case of shareware).</rdfs:comment>
        <rdfs:subClassOf rdf:resource="govLayer1#TechnologyProvider"/>
        <rdfs:isDefinedBy rdf:resource="https://en.wikipedia.org/wiki/Software_publisher"/>
    </owl:Class>

    <owl:Class rdf:about="techLayer3#Issuer">
        <rdfs:label>Issuer</rdfs:label>
        <rdfs:comment>A role an agent performs to package and digitally sign a set of claims, typically in the form of a digital credential, and transmit them to a holder.</rdfs:comment>
        <rdfs:subClassOf rdf:resource="techLayer3#Actor"/>
        <rdfs:isDefinedBy rdf:resource="https://glossary.trustoverip.org/#term:issuer"/>
    </owl:Class>

    <owl:Class rdf:about="techLayer3#Verifier">
        <rdfs:label>Verifier</rdfs:label>
        <rdfs:comment>A role an agent performs to perform verification of one or more proofs of the claims in a digital credential or other verifiable data.</rdfs:comment>
        <rdfs:subClassOf rdf:resource="techLayer3#Actor"/>
        <rdfs:isDefinedBy rdf:resource="https://glossary.trustoverip.org/#term:verifier"/>
    </owl:Class>
      
    <owl:Class rdf:about="techLayer3#Credential">
        <rdfs:label>Credential</rdfs:label>
        <rdfs:comment>A container of claims describing one or more subjects. A credential is generated by the issuer of the credential and given to the holder of the credential. A credential typically includes a signature or some other means of proving its authenticity. A credential may be either a physical credential or a digital credential.</rdfs:comment>
        <rdfs:isDefinedBy rdf:resource="https://glossary.trustoverip.org/#term:credential"/>
    </owl:Class>

    <owl:Class rdf:about="governance#AdministeringAuthority">
        <rdfs:label>Administering authority</rdfs:label>
        <rdfs:comment>A legal entity delegated by a governing body to administer the operation of a governance framework and governed infrastructure for a digital trust ecosystem, such as one or more trust registries.</rdfs:comment>
        <rdfs:subClassOf rdf:resource="techLayer4#Entity"/>
        <rdfs:isDefinedBy rdf:resource="https://glossary.trustoverip.org/#term:administering-authority"/>
    </owl:Class>

    <owl:Class rdf:about="govLayer1#TechnicalStandard">
        <rdfs:label>Technical standard</rdfs:label>
        <rdfs:comment>A technical standard is an established norm or requirement for a repeatable technical task which is applied to a common and repeated use of rules, conditions, guidelines or characteristics for products or related processes and production methods, and related management systems practices.</rdfs:comment>
        <rdfs:isDefinedBy rdf:resource="https://en.wikipedia.org/wiki/Technical_standard"/>
    </owl:Class>



    <!-- ******************************* -->
    <!-- ********* Instance ************ -->
    <!-- ******************************* -->



</rdf:RDF>
