<?xml version="1.0"?>
<rdf:RDF xmlns="http://example.org/govLayer3#"
    xml:base="http://example.org/govLayer3"
    xmlns:rdf="http://www.w3.org/1999/02/22-rdf-syntax-ns#"
    xmlns:owl="http://www.w3.org/2002/07/owl#"
    xmlns:rdfs="http://www.w3.org/2000/01/rdf-schema#"
    xmlns:xsd="http://www.w3.org/2001/XMLSchema#">



    <!-- ********************************************************************************************* -->
    <!-- *******************  All rights reserved to Cristian Lepore ********************************* -->
    <!-- ************************* Gov layer 3 of the ToIP model ************************************* -->
    <!-- ******** Definitions comes from the ToIP Glossary: https://glossary.trustoverip.org/ ******** -->
    <!-- ********************************************************************************************* -->

    <owl:Ontology rdf:about="http://example.org/govLayer3#">
        <rdfs:comment>Ontology representing the governance Layer 3 of the ToIP stack.</rdfs:comment>
    </owl:Ontology>



    <!-- ******************************* -->
    <!-- ********* Class *************** -->
    <!-- ******************************* -->

    <owl:Class rdf:about="govLayer3#Insurer">
        <rdfs:label>Insurer</rdfs:label>
        <rdfs:comment>A person or company that insures someone or something.</rdfs:comment>
        <rdfs:isDefinedBy rdf:resource="https://dictionary.cambridge.org/dictionary/english/insurer"/>
    </owl:Class>

    <owl:Class rdf:about="govLayer3#RiskLevel">
        <rdfs:label>Risk level</rdfs:label>
        <rdfs:comment></rdfs:comment>
    </owl:Class>



    <!-- ******************************* -->
    <!-- ********* Relation ************ -->
    <!-- ******************************* -->

    <owl:ObjectProperty rdf:about="govLayer3#adoptsTechnicalStandard">
        <rdfs:domain rdf:resource="govLayer1#TechnologyProvider"/>
        <rdfs:range rdf:resource="govLayer1#TechnicalStandard"/>
        <rdfs:label>adopts</rdfs:label>
        <rdfs:comment>The technology provider adopts technical standards.</rdfs:comment>
    </owl:ObjectProperty>

    <owl:ObjectProperty rdf:about="govLayer3#identifiesRiskLevel">
        <rdfs:domain rdf:resource="governance#ControlledDocument"/>
        <rdfs:range rdf:resource="govLayer3#RiskLevel"/>
        <rdfs:label>identifies</rdfs:label>
        <rdfs:comment>The process of identifying risks to organizational operations (including mission, functions, image, reputation), organizational assets, individuals, other organizations, and the overall ecosystem, resulting from the operation of an information system. Risk assessment is part of risk management, incorporates threat and vulnerability analyses, and considers risk mitigations provided by security controls planned or in place.</rdfs:comment>
        <rdfs:isDefinedBy rdf:resource="https://glossary.trustoverip.org/#term:risk-assessment"/>
    </owl:ObjectProperty>

    <owl:ObjectProperty rdf:about="govLayer3#issuerConsultsAuthoritativeSource">
        <rdfs:domain rdf:resource="techLayer3#Issuer"/>
        <rdfs:range rdf:resource="govLayer3#AuthoritativeSource"/>
        <rdfs:label>consults</rdfs:label>
        <rdfs:comment>The issuer queries the authoritative source of information, for example to discover the credential schemes and attributes. Paper: Lepore, Cristian, Romain Laborde, and Jessica Eynard. Aligning eIDAS and Trust Over IP: A Mapping Approach. Proceedings of the 19th International Conference on Availability, Reliability and Security. 2024.</rdfs:comment>
        <rdfs:isDefinedBy rdf:resource="https://doi.org/10.1007/978-3-031-89350-6_4"/>
    </owl:ObjectProperty>

    <owl:ObjectProperty rdf:about="govLayer3#registersIssuer">
        <rdfs:domain rdf:resource="govLayer3#Registrant"/>
        <rdfs:range rdf:resource="techLayer3#Issuer"/>
        <rdfs:label>registers</rdfs:label>
        <rdfs:comment>The party submitting a registration record to a registry.</rdfs:comment>
        <rdfs:isDefinedBy rdf:resource="https://glossary.trustoverip.org/#term:registrant"/>
    </owl:ObjectProperty>

    <owl:ObjectProperty rdf:about="govLayer3#executesControlledDocument">
        <rdfs:domain rdf:resource="govLayer3#Insurer"/>
        <rdfs:range rdf:resource="governance#ControlledDocument"/>
        <rdfs:label>executes</rdfs:label>
        <rdfs:comment>The insurer executes the risk assessment.</rdfs:comment>
    </owl:ObjectProperty>



    <!-- ******************************* -->
    <!-- ********* Attribute *********** -->
    <!-- ******************************* -->

    <owl:DatatypeProperty rdf:about="govLayer1#open">
        <rdfs:domain rdf:resource="govLayer1#TechnicalStandard"/>
        <rdfs:range rdf:resource="http://www.w3.org/2001/XMLSchema#boolean"/>
        <rdfs:label>open</rdfs:label>
        <rdfs:comment>Indicates whether the technical standards are open to public review and comment.</rdfs:comment>
    </owl:DatatypeProperty>


    <!-- ******************************* -->
    <!-- * Connection with other Layer * -->
    <!-- ******************************* -->
    
    <owl:Class rdf:about="techLayer3#Holder">
        <rdfs:label>Holder</rdfs:label>
        <rdfs:comment>A role an agent performs by serving as the controller of the cryptographic keys and digital credentials in a digital wallet. The holder makes issuance requests for credentials and responds to presentation requests for credentials. A holder is usually, but not always, a subject of the credentials they are holding.</rdfs:comment>
        <rdfs:subClassOf rdf:resource="techLayer3#Actor"/>
        <rdfs:isDefinedBy rdf:resource="https://glossary.trustoverip.org/#term:holder"/>
    </owl:Class>

    <owl:Class rdf:about="techLayer3#Verifier">
        <rdfs:label>Verifier</rdfs:label>
        <rdfs:comment>A role an agent performs to perform verification of one or more proofs of the claims in a digital credential or other verifiable data.</rdfs:comment>
        <rdfs:subClassOf rdf:resource="techLayer3#Actor"/>
        <rdfs:isDefinedBy rdf:resource="https://glossary.trustoverip.org/#term:verifier"/>
    </owl:Class>



    <!-- ******************************* -->
    <!-- ********* Instance ************ -->
    <!-- ******************************* -->



</rdf:RDF>
