<?xml version="1.0"?>
<rdf:RDF xmlns="http://example.org/techLayer3#"
      xml:base="http://example.org/techLayer3"
      xmlns:rdf="http://www.w3.org/1999/02/22-rdf-syntax-ns#"
      xmlns:owl="http://www.w3.org/2002/07/owl#"
      xmlns:rdfs="http://www.w3.org/2000/01/rdf-schema#"
      xmlns:xsd="http://www.w3.org/2001/XMLSchema#">
      
      <!-- ********************************************************************************************* -->
      <!-- *******************  All rights reserved to Cristian Lepore ********************************* -->
      <!-- ************************* Tech layer 3 of the ToIP model ************************************ -->
      <!-- ******** Definitions comes from the ToIP Glossary: https://glossary.trustoverip.org/ ******** -->
      <!-- ********************************************************************************************* -->  

      <owl:Ontology rdf:about="http://example.org/techLayer3#">
            <rdfs:comment>Ontology representing the tech Layer 3 of the ToIP stack.</rdfs:comment>
      </owl:Ontology>



      <!-- ******************************* -->
      <!-- ********* Class *************** -->
      <!-- ******************************* -->

      <owl:Class rdf:about="techLayer3#Attribute">
            <rdfs:label>Attribute</rdfs:label>
            <rdfs:comment>An identifiable set of data that describes an entity, which is the subject of the attribute.</rdfs:comment>
            <rdfs:isDefinedBy rdf:resource="https://glossary.trustoverip.org/#term:attributes"/>
      </owl:Class>

      <owl:Class rdf:about="techLayer3#Actor">
            <rdfs:label>Actor</rdfs:label>
            <rdfs:comment>An entity that can act (do things/execute actions), e.g. people, machines, but not organizations. A digital agent can serve as an actor acting on behalf of its principal.</rdfs:comment>
            <rdfs:subClassOf rdf:resource="techLayer4#Party"/>
            <rdfs:isDefinedBy rdf:resource="https://glossary.trustoverip.org/#term:actor"/>
      </owl:Class>

      <owl:Class rdf:about="techLayer3#Credential">
            <rdfs:label>Credential</rdfs:label>
            <rdfs:comment>A credential in digital form that is signed with a digital signature and held in a digital wallet. A digital credential is issued to a holder by an issuer; a proof of the credential is presented by the holder to a verifier.</rdfs:comment>
            <rdfs:isDefinedBy rdf:resource="https://glossary.trustoverip.org/#term:digital-credential"/>
      </owl:Class>

      <owl:Class rdf:about="techLayer3#VC">
            <rdfs:label>Verifiable credential</rdfs:label>
            <rdfs:comment>A standard data model and representation format for cryptographically-verifiable digital credentials as defined by the W3C Verifiable Credentials Data Model Specification.</rdfs:comment>
            <rdfs:subClassOf rdf:resource="techLayer3#Credential"/>
            <rdfs:isDefinedBy rdf:resource="https://glossary.trustoverip.org/#term:verifiable-credential"/>
      </owl:Class>
      <!--
      <owl:Class rdf:about="#ChainedCredential">
            <rdfs:label>Chained credential</rdfs:label>
            <rdfs:comment>Two or more credentials linked together to create a trust chain between the credentials that is cryptographically verifiable.</rdfs:comment>
            <rdfs:subClassOf rdf:resource="techLayer3#Credential"/>
            <rdfs:isDefinedBy rdf:resource="https://glossary.trustoverip.org/#term:chained-credentials"/>
      </owl:Class>
      -->
      <owl:Class rdf:about="techLayer3#Proof">
            <rdfs:label>Proof</rdfs:label>
            <rdfs:comment>A digital object that enables cryptographic verification of either: a) the claims from one or more digital credentials, or b) facts about claims that do not reveal the data itself (e.g., proof of the subject being over/under a specific age without revealing a birthdate).</rdfs:comment>
            <rdfs:isDefinedBy rdf:resource="https://glossary.trustoverip.org/#term:proof"/>
      </owl:Class>

      <owl:Class rdf:about="techLayer3#ZeroKnowledgeProof">
            <rdfs:label>Zero-knowledge proof</rdfs:label>
            <rdfs:comment>A specific kind of cryptographic proof that proves facts about data to a verifier without revealing the underlying data itself. A common example is proving that a person is over or under a specific age without revealing the personâ€™s exact birthdate.</rdfs:comment>
            <rdfs:subClassOf rdf:resource="techLayer3#Proof"/>
            <rdfs:isDefinedBy rdf:resource="https://glossary.trustoverip.org/#term:zero-knowledge-proof"/>
      </owl:Class>

      <owl:Class rdf:about="techLayer3#Issuer">
            <rdfs:label>Issuer</rdfs:label>
            <rdfs:comment>A role an agent performs to package and digitally sign a set of claims, typically in the form of a digital credential, and transmit them to a holder.</rdfs:comment>
            <rdfs:subClassOf rdf:resource="techLayer3#Actor"/>
            <rdfs:isDefinedBy rdf:resource="https://glossary.trustoverip.org/#term:issuer"/>
      </owl:Class>

      <owl:Class rdf:about="techLayer3#Holder">
            <rdfs:label>Holder</rdfs:label>
            <rdfs:comment>A role an agent performs by serving as the controller of the cryptographic keys and digital credentials in a digital wallet. The holder makes issuance requests for credentials and responds to presentation requests for credentials. A holder is usually, but not always, a subject of the credentials they are holding.</rdfs:comment>
            <rdfs:subClassOf rdf:resource="techLayer3#Actor"/>
            <rdfs:isDefinedBy rdf:resource="https://glossary.trustoverip.org/#term:holder"/>
      </owl:Class>

      <owl:Class rdf:about="techLayer3#Verifier">
            <rdfs:label>Verifier</rdfs:label>
            <rdfs:comment>A role an agent performs to perform verification of one or more proofs of the claims in a digital credential or other verifiable data.</rdfs:comment>
            <rdfs:subClassOf rdf:resource="techLayer3#Actor"/>
            <rdfs:isDefinedBy rdf:resource="https://glossary.trustoverip.org/#term:verifier"/>
      </owl:Class>

      <owl:Class rdf:about="techLayer3#TrustTaskProtocol">
            <rdfs:label>Trust Task Protocol</rdfs:label>
            <rdfs:comment>A ToIP Layer 3 protocol that implements a specific trust task on behalf of a trust application operating at ToIP Layer 4.</rdfs:comment>
            <rdfs:isDefinedBy rdf:resource="https://glossary.trustoverip.org/#term:trust-task-protocol"/>
      </owl:Class>

      <owl:Class rdf:about="techLayer3#TrustRegistryProtocol">
            <rdfs:label>Trust registry protocol</rdfs:label>
            <rdfs:comment>The open standard trust task protocol defined by the ToIP Foundation to perform the trust task of querying a trust registry. The ToIP Trust Registry Protocol operates at Layer 3 of the ToIP stack.</rdfs:comment>
            <rdfs:subClassOf rdf:resource="techLayer3#TrustTaskProtocol"/>
            <rdfs:isDefinedBy rdf:resource="https://glossary.trustoverip.org/#term:toip-trust-registry-protocol"/>
      </owl:Class>

      <owl:Class rdf:about="techLayer3#CredentialExchangeProtocol">
            <rdfs:label>Credential exchange protocol</rdfs:label>
            <rdfs:comment>Credential exchange protocol governs the secure exchange of verifiable credentials between parties, including specialized sub-protocols.</rdfs:comment>
            <rdfs:subClassOf rdf:resource="techLayer3#TrustTaskProtocol"/>
            <rdfs:isDefinedBy rdf:resource="https://trustoverip.github.io/TechArch/"/>
      </owl:Class>

      <owl:Class rdf:about="techLayer3#CredentialIssuanceProtocol">
            <rdfs:label>Credential issuance protocol</rdfs:label>
            <rdfs:comment>Credential issuance protocol, for issuing credentials to a holder.</rdfs:comment>
            <rdfs:subClassOf rdf:resource="techLayer3#CredentialExchangeProtocol"/>
            <rdfs:isDefinedBy rdf:resource="https://trustoverip.github.io/TechArch/"/>
      </owl:Class>

      <owl:Class rdf:about="techLayer3#ProofPresentationProtocol">
            <rdfs:label>Proof presentation protocol</rdfs:label>
            <rdfs:comment>Proof presentation protocol, for presenting verifiable proofs derived from credentials.</rdfs:comment>
            <rdfs:subClassOf rdf:resource="techLayer3#CredentialExchangeProtocol"/>
            <rdfs:isDefinedBy rdf:resource="https://trustoverip.github.io/TechArch/"/>
      </owl:Class>

      <owl:Class rdf:about="techLayer3#CredentialOfferProtocol">
            <rdfs:label>Credential offer protocol</rdfs:label>
            <rdfs:comment>Credential offer protocol, which initiates the issuance process by offering a credential.</rdfs:comment>
            <rdfs:subClassOf rdf:resource="techLayer3#CredentialIssuanceProtocol"/>
            <rdfs:isDefinedBy rdf:resource="https://trustoverip.github.io/TechArch/"/>
      </owl:Class>

      <owl:Class rdf:about="techLayer3#IdentifierExchangeProtocol">
            <rdfs:label>Identifier exchange protocol</rdfs:label>
            <rdfs:comment></rdfs:comment>
            <rdfs:subClassOf rdf:resource="techLayer3#TrustTaskProtocol"/>
      </owl:Class>

      <owl:Class rdf:about="techLayer3#MessagingProtocol">
            <rdfs:label>Messaging protocol</rdfs:label>
            <rdfs:comment>Messaging protocol ensures confidential and authenticated communication between agents.</rdfs:comment>
            <rdfs:subClassOf rdf:resource="techLayer3#TrustTaskProtocol"/>
            <rdfs:isDefinedBy rdf:resource="https://trustoverip.github.io/TechArch/"/>
      </owl:Class>

      <owl:Class rdf:about="techLayer3#RevocationNotificationProtocol">
            <rdfs:label>Revocation Notification Protocol</rdfs:label>
            <rdfs:comment>Revocation Notification Protocol informs relevant parties about the revocation of credentials, maintaining trust in dynamic environments.</rdfs:comment>
            <rdfs:subClassOf rdf:resource="techLayer3#TrustTaskProtocol"/>
            <rdfs:isDefinedBy rdf:resource="https://trustoverip.github.io/TechArch/"/>
      </owl:Class>

      <owl:Class rdf:about="techLayer3#OutOfBandProtocol">
            <rdfs:label>Out-of-Band Protocol</rdfs:label>
            <rdfs:comment>Used to initiate the interaction without a persistence connection.</rdfs:comment>
            <rdfs:subClassOf rdf:resource="techLayer3#TrustTaskProtocol"/>
      </owl:Class>

      <owl:Class rdf:about="techLayer3#DataFormat">
            <rdfs:label>Data format</rdfs:label>
            <rdfs:comment>The data format of credentials and proofs.</rdfs:comment>
      </owl:Class>




      <!-- ******************************* -->
      <!-- ********* Attribute *********** -->
      <!-- ******************************* -->




      <!-- ******************************* -->
      <!-- ********* Relation ************ -->
      <!-- ******************************* -->

      <owl:ObjectProperty rdf:about="techLayer3#containsAttribute">
            <rdfs:domain rdf:resource="techLayer3#Proof"/>
            <rdfs:range rdf:resource="techLayer3#Attribute"/>
            <rdfs:label>contains</rdfs:label>
      </owl:ObjectProperty>

      <owl:ObjectProperty rdf:about="techLayer3#encodesAttribute">
            <rdfs:domain rdf:resource="techLayer3#Credential"/>
            <rdfs:range rdf:resource="techLayer3#Attribute"/>
            <rdfs:label>encodes</rdfs:label>
      </owl:ObjectProperty>

      <owl:ObjectProperty rdf:about="techLayer3#usesTrustTaskProtocol">
            <rdfs:domain rdf:resource="techLayer3#Actor"/>
            <rdfs:range rdf:resource="techLayer3#TrustTaskProtocol"/>
            <rdfs:label>uses</rdfs:label>
            <rdfs:comment>The open standard trust task protocol defined by the ToIP Foundation to perform the trust task of querying a trust registry. The ToIP Trust Registry Protocol operates at Layer 3 of the ToIP stack.</rdfs:comment>
            <rdfs:isDefinedBy rdf:resource="https://glossary.trustoverip.org/#term:toip-trust-registry-protocol"/>
      </owl:ObjectProperty>

      <owl:ObjectProperty rdf:about="techLayer3#consultsRegistry">
            <rdfs:domain rdf:resource="techLayer3#TrustRegistryProtocol"/>
            <rdfs:range rdf:resource="techLayer1#Registry"/>
            <rdfs:label>consults</rdfs:label>
            <rdfs:comment>The open standard trust task protocol defined by the ToIP Foundation to perform the trust task of querying a trust registry. The ToIP Trust Registry Protocol operates at Layer 3 of the ToIP stack.</rdfs:comment>
            <rdfs:isDefinedBy rdf:resource="https://glossary.trustoverip.org/#term:toip-trust-registry-protocol"/>
      </owl:ObjectProperty>

      <owl:ObjectProperty rdf:about="techLayer3#implementsTrustTask">
            <rdfs:domain rdf:resource="techLayer3#TrustTaskProtocol"/>
            <rdfs:range rdf:resource="techLayer4#TrustTask"/>
            <rdfs:label>implements</rdfs:label>
            <rdfs:comment>A ToIP Layer 3 protocol that implements a specific trust task on behalf of a trust application operating at ToIP Layer 4.</rdfs:comment>
            <rdfs:isDefinedBy rdf:resource="https://glossary.trustoverip.org/#term:trust-task-protocol"/>
      </owl:ObjectProperty>

      <owl:ObjectProperty rdf:about="techLayer3#agencyOfUserAgent">
            <rdfs:domain rdf:resource="techLayer3#Actor"/>
            <rdfs:range rdf:resource="techLayer2#UserAgent"/>
            <rdfs:label>agency of</rdfs:label>
            <rdfs:comment>An entity that can act (do things/execute actions), e.g. people, machines, but not organizations. A digital agent can serve as an actor acting on behalf of its principal.</rdfs:comment>
            <rdfs:isDefinedBy rdf:resource="https://glossary.trustoverip.org/#term:actor"/>
      </owl:ObjectProperty>

      <owl:ObjectProperty rdf:about="techLayer3#issuanceCredential">
            <rdfs:domain rdf:resource="techLayer3#CredentialExchangeProtocol"/>
            <rdfs:range rdf:resource="techLayer3#Credential"/>
            <rdfs:label>issuance</rdfs:label>
            <rdfs:comment>The action of an issuer producing and transmitting a digital credential to a holder. A holder may request issuance by submitting an issuance request.</rdfs:comment>
            <rdfs:isDefinedBy rdf:resource="https://glossary.trustoverip.org/#term:issuance"/>
      </owl:ObjectProperty>

      <owl:ObjectProperty rdf:about="techLayer3#presentationProof">
            <rdfs:domain rdf:resource="techLayer3#CredentialExchangeProtocol"/>
            <rdfs:range rdf:resource="techLayer3#Proof"/>
            <rdfs:label>presentation</rdfs:label>
            <rdfs:comment>A verifiable message that a holder may send to a verifier containing proofs of one or more claims derived from one or more digital credentials from one or more issuers as a response to a specific presentation request from a  verifier.</rdfs:comment>
            <rdfs:isDefinedBy rdf:resource="https://glossary.trustoverip.org/#term:presentation"/>
      </owl:ObjectProperty>

      <owl:ObjectProperty rdf:about="techLayer3#supportsDataFormat">
            <rdfs:domain rdf:resource="techLayer3#TrustTaskProtocol"/>
            <rdfs:range rdf:resource="techLayer3#DataFormat"/>
            <rdfs:label>supports</rdfs:label>
            <rdfs:comment>A credential and a proof support a specific data format.</rdfs:comment>
      </owl:ObjectProperty>



      <!-- ******************************* -->
      <!-- ******** Constraints ********** -->
      <!-- ******************************* -->

      <!-- Issuer, holder, verifier are disjoint -->
      <owl:AllDisjointClasses>
            <owl:members rdf:parseType="Collection">
                  <rdf:Description rdf:about="techLayer3#Issuer"/>
                  <rdf:Description rdf:about="techLayer3#Holder"/>
                  <rdf:Description rdf:about="techLayer3#Verifier"/>
            </owl:members>
      </owl:AllDisjointClasses>



      <!-- ******************************* -->
      <!-- * Connection with other Layer * -->
      <!-- ******************************* -->

      <owl:Class rdf:about="techLayer4#Party">
            <rdfs:label>Party</rdfs:label>
            <rdfs:comment>An entity that sets its objectives, maintains its knowledge, and uses that knowledge to pursue its objectives in an autonomous (sovereign) manner. Natural persons and organizations are the typical examples.</rdfs:comment>
            <rdfs:subClassOf rdf:resource="techLayer4#Entity"/>
            <rdfs:isDefinedBy rdf:resource="https://glossary.trustoverip.org/#term:party"/>
      </owl:Class>

      <owl:Class rdf:about="techLayer1#Registry">
            <rdfs:label>Registry</rdfs:label>
            <rdfs:comment>A specialized database of records that serves as an authoritative source of information about entities.</rdfs:comment>
            <rdfs:subClassOf rdf:resource="techLayer1#DigitalTrustUtility"/>
            <rdfs:isDefinedBy rdf:resource="https://glossary.trustoverip.org/#term:registry"/>
      </owl:Class>

      <owl:Class rdf:about="techLayer2#UserAgent">
            <rdfs:label>User Agent</rdfs:label>
            <rdfs:comment>A software agent that is used directly by the end-user as the principal. Browsers, email clients, and digital wallets are all examples of user agents.</rdfs:comment>
            <rdfs:isDefinedBy rdf:resource="https://glossary.trustoverip.org/#term:user-agent"/>
      </owl:Class>

      <owl:Class rdf:about="techLayer4#TrustTask">
            <rdfs:label>Trust Task</rdfs:label>
            <rdfs:comment>A specific task that involves establishing, verifying, or maintaining trust relationships or exchanging verifiable messages or verifiable data that can be performed on behalf of a trust application by a trust task protocol at Layer 3 of the ToIP stack.</rdfs:comment>
            <rdfs:isDefinedBy rdf:resource="https://glossary.trustoverip.org/#term:trust-task"/>
      </owl:Class>



      <!-- ******************************* -->
      <!-- ********* Instance ************ -->
      <!-- ******************************* -->





</rdf:RDF>
