<?xml version="1.0"?>
<rdf:RDF xmlns="http://example.org/techLayer1#"
     xml:base="http://example.org/techLayer1"
     xmlns:rdf="http://www.w3.org/1999/02/22-rdf-syntax-ns#"
     xmlns:owl="http://www.w3.org/2002/07/owl#"
     xmlns:rdfs="http://www.w3.org/2000/01/rdf-schema#"
     xmlns:xsd="http://www.w3.org/2001/XMLSchema#">

     <!-- ********************************************************************************************* -->
     <!-- *******************  All rights reserved to Cristian Lepore ********************************* -->
     <!-- ************************* Tech layer 1 of the ToIP model ************************************ -->
     <!-- ******** Definitions comes from the ToIP Glossary: https://glossary.trustoverip.org/ ******** -->
     <!-- ********************************************************************************************* -->

     <owl:Ontology rdf:about="http://example.org/techLayer1#">
          <rdfs:comment>Ontology representing the tech Layer 1 of the ToIP stack.</rdfs:comment>
     </owl:Ontology>



     <!-- ******************************* -->
     <!-- ********* Class *************** -->
     <!-- ******************************* -->

     <owl:Class rdf:about="techLayer1#DigitalTrustUtility">
          <rdfs:label>Digital trust utility</rdfs:label>
          <rdfs:comment>An information system, network, distributed database, or blockchain designed to provide one or more supporting services to higher level components of decentralized digital trust infrastructure. In the ToIP stack, digital trust utilities are at Layer 1. A verifiable data registry is one type of digital trust utility.</rdfs:comment>
          <rdfs:isDefinedBy rdf:resource="https://glossary.trustoverip.org/#term:digital-trust-utility"/>
     </owl:Class>

     <owl:Class rdf:about="techLayer1#Registry">
          <rdfs:label>Registry</rdfs:label>
          <rdfs:comment>A specialized database of records that serves as an authoritative source of information about entities.</rdfs:comment>
          <rdfs:subClassOf rdf:resource="techLayer1#DigitalTrustUtility"/>
          <rdfs:isDefinedBy rdf:resource="https://glossary.trustoverip.org/#term:registry"/>
     </owl:Class>

     <owl:Class rdf:about="techLayer1#TrustRegistry">
          <rdfs:label>Trust Registry</rdfs:label>
          <rdfs:comment>A registry that serves as an authoritative source for trust graphs or other governed information describing one or more trust communities. A trust registry is typically authorized by a governance framework.</rdfs:comment>
          <rdfs:subClassOf rdf:resource="techLayer1#Registry"/>
          <rdfs:isDefinedBy rdf:resource="https://glossary.trustoverip.org/#term:trust-registry"/>
     </owl:Class>

     <owl:Class rdf:about="techLayer1#TrustList">
          <rdfs:label>Trust List</rdfs:label>
          <rdfs:comment>A one-dimensional trust graph in which an authoritative source publishes a list of entities that are trusted in a specific trust context. A trust list can be considered a simplified form of a trust registry.</rdfs:comment>
          <rdfs:subClassOf rdf:resource="techLayer1#TrustRegistry"/>
          <rdfs:isDefinedBy rdf:resource="https://glossary.trustoverip.org/#term:trust-list"/>
     </owl:Class>

     <owl:Class rdf:about="techLayer1#VDR">
          <rdfs:label>VDR</rdfs:label>
          <rdfs:comment>A registry that facilitates the creation, verification, updating, and/or deactivation of decentralized identifiers and DID documents. A verifiable data registry may also be used for other cryptographically-verifiable data structures such as verifiable credentials.</rdfs:comment>
          <rdfs:subClassOf rdf:resource="techLayer1#Registry"/>
          <rdfs:isDefinedBy rdf:resource="https://glossary.trustoverip.org/#term:verifiable-data-registry"/>
     </owl:Class>

     <owl:Class rdf:about="techLayer1#ArchitectureType">
          <rdfs:label>Architecture type</rdfs:label>
          <rdfs:comment>The type of architecture of a registry.</rdfs:comment>
          <rdfs:isDefinedBy rdf:resource="https://trustoverip.org/permalink/ToIP-Technical-Architecture-Specification-V1.0-PR1-2022-11-14.pdf"/>
     </owl:Class>

     <owl:Class rdf:about="techLayer1#CentralizedArchitecture">
          <rdfs:label>Centralized architecture</rdfs:label>
          <rdfs:comment>A centralized architecture of a registry.</rdfs:comment>
          <rdfs:subClassOf rdf:resource="techLayer1#ArchitectureType"/>
     </owl:Class>

     <owl:Class rdf:about="techLayer1#DecentralizedArchitecture">
          <rdfs:label>Decentralized architecture</rdfs:label>
          <rdfs:comment>A decentralized architecture of registries.</rdfs:comment>
          <rdfs:subClassOf rdf:resource="techLayer1#ArchitectureType"/>
     </owl:Class>

     <owl:Class rdf:about="techLayer1#Federated">
          <rdfs:label>Federated</rdfs:label>
          <rdfs:comment>A group of organizations that collaborate to establish a common trust framework or governance framework for the exchange of identity data in a federated identity system.</rdfs:comment>
          <rdfs:subClassOf rdf:resource="techLayer1#ArchitectureType"/>
          <rdfs:isDefinedBy rdf:resource="https://glossary.trustoverip.org/#term:federation"/>
     </owl:Class>

     <owl:Class rdf:about="techLayer1#Identifier">
          <rdfs:label>Identifier</rdfs:label>
          <rdfs:comment>A single attribute—typically a character string—that uniquely identifies an entity within a specific context (which may be a global context). Examples include the name of a party, the URL of an organization, or a serial number for a man-made thing.</rdfs:comment>
          <rdfs:subClassOf rdf:resource="techLayer1#DigitalTrustUtility"/>
          <rdfs:isDefinedBy rdf:resource="https://glossary.trustoverip.org/#term:identifier"/>
     </owl:Class>

     <owl:Class rdf:about="techLayer1#VID">
          <rdfs:label>VID</rdfs:label>
          <rdfs:comment>An identifier over which the controller can provide cryptographic proof of control. Each type of VID defines a specific means for discovering the public key, network endpoints, or other metadata necessary to prove control. Decentralized identifiers (DIDs) are a W3C standard for VIDs. VIDs are the cryptographically verifiable identifiers used in the ToIP stack.</rdfs:comment>
          <rdfs:subClassOf rdf:resource="techLayer1#Identifier"/>
          <rdfs:isDefinedBy rdf:resource="https://glossary.trustoverip.org/#term:verifiable-identifier"/>
     </owl:Class>

     <owl:Class rdf:about="techLayer1#Non-VID">
          <rdfs:label>Non-VID</rdfs:label>
          <rdfs:comment>An identifier that is not tied to a cryptographic proof of control. This identifier is not part of the ToIP model.</rdfs:comment>
          <rdfs:subClassOf rdf:resource="techLayer1#Identifier"/>
          <rdfs:isDefinedBy rdf:resource="https://trustoverip.org/permalink/ToIP-Technical-Architecture-Specification-V1.0-PR1-2022-11-14.pdf"/>
     </owl:Class>

     <owl:Class rdf:about="techLayer1#CentralizedIdentifier">
          <rdfs:label>Centralized identifier</rdfs:label>
          <rdfs:comment>A VID that requires a centralized registry.</rdfs:comment>
          <rdfs:subClassOf rdf:resource="techLayer1#VID"/>
          <rdfs:isDefinedBy rdf:resource="https://trustoverip.org/permalink/ToIP-Technical-Architecture-Specification-V1.0-PR1-2022-11-14.pdf"/>
     </owl:Class>

     <owl:Class rdf:about="techLayer1#DecentralizedIdentifier">
          <rdfs:label>Decentralized identifier</rdfs:label>
          <rdfs:comment>A VID that requires a decentralized registry.</rdfs:comment>
          <rdfs:subClassOf rdf:resource="techLayer1#VID"/>
          <rdfs:isDefinedBy rdf:resource="https://trustoverip.org/permalink/ToIP-Technical-Architecture-Specification-V1.0-PR1-2022-11-14.pdf"/>
     </owl:Class>

     <owl:Class rdf:about="techLayer1#SelfCertifyingIdentifier">
          <rdfs:label>Self-certifying (Autonomic) identifier</rdfs:label>
          <rdfs:comment>A subclass of verifiable identifier (VID) that is cryptographically verifiable without the need to rely on any third party for verification because the identifier is cryptographically bound to the cryptographic keys from which it was generated.</rdfs:comment>
          <rdfs:subClassOf rdf:resource="techLayer1#DecentralizedIdentifier"/>
          <rdfs:isDefinedBy rdf:resource="https://glossary.trustoverip.org/#term:self-certifying-identifier"/>
     </owl:Class>

     <owl:Class rdf:about="techLayer1#Non-SelfCertifyingIdentifier">
          <rdfs:label>Non-Self Certifying identifier</rdfs:label>
          <rdfs:comment>A subclass of verifiable identifier (VID) that is not self generated by the entity.</rdfs:comment>
          <rdfs:subClassOf rdf:resource="techLayer1#DecentralizedIdentifier"/>
          <rdfs:isDefinedBy rdf:resource="https://trustoverip.org/permalink/ToIP-Technical-Architecture-Specification-V1.0-PR1-2022-11-14.pdf"/>
     </owl:Class>

     <owl:Class rdf:about="techLayer1#Metadata">
          <rdfs:label>Metadata</rdfs:label>
          <rdfs:comment>Information describing the characteristics of data including, for example, structural metadata describing data structures (e.g., data format, syntax, and semantics) and descriptive metadata describing data contents (e.g., information security labels).</rdfs:comment>
          <rdfs:isDefinedBy rdf:resource="https://glossary.trustoverip.org/#term:metadata"/>
     </owl:Class>



     <!-- ******************************* -->
     <!-- ********* Attribute *********** -->
     <!-- ******************************* -->

     <owl:DatatypeProperty rdf:about="techLayer1#discoverable">
          <rdfs:domain rdf:resource="techLayer1#VID"/>
          <rdfs:range rdf:resource="http://www.w3.org/2001/XMLSchema#boolean"/>
          <rdfs:label>discoverable</rdfs:label>
          <rdfs:comment>A verifiable identifier may be discoverable. [L2.8]</rdfs:comment>
          <rdfs:isDefinedBy rdf:resource="https://trustoverip.org/permalink/ToIP-Technical-Architecture-Specification-V1.0-PR1-2022-11-14.pdf"/>
     </owl:DatatypeProperty>

     <owl:DatatypeProperty rdf:about="techLayer1#portable">
          <rdfs:domain rdf:resource="techLayer1#VID"/>
          <rdfs:range rdf:resource="http://www.w3.org/2001/XMLSchema#boolean"/>
          <rdfs:label>portable</rdfs:label>
          <rdfs:comment>A verifiable identifier should be portable. [L2.5]</rdfs:comment>
          <rdfs:isDefinedBy rdf:resource="https://trustoverip.org/permalink/ToIP-Technical-Architecture-Specification-V1.0-PR1-2022-11-14.pdf"/>
     </owl:DatatypeProperty>

     <owl:DatatypeProperty rdf:about="techLayer1#persistent">
          <rdfs:domain rdf:resource="techLayer1#VID"/>
          <rdfs:range rdf:resource="http://www.w3.org/2001/XMLSchema#boolean"/>
          <rdfs:label>persistent</rdfs:label>
          <rdfs:comment>The identifier never needs to change.</rdfs:comment>
          <rdfs:isDefinedBy rdf:resource="https://trustoverip.org/wp-content/uploads/ToIP-Governance-Architecture-Specification-V1.0-2021-12-21.pdf"/>
     </owl:DatatypeProperty>

     <owl:DatatypeProperty rdf:about="techLayer1#permissioned">
          <rdfs:domain rdf:resource="techLayer1#Registry"/>
          <rdfs:range rdf:resource="http://www.w3.org/2001/XMLSchema#boolean"/>
          <rdfs:label>permissioned</rdfs:label>
          <rdfs:comment></rdfs:comment>
     </owl:DatatypeProperty>

     <owl:DatatypeProperty rdf:about="techLayer1#permissionless">
          <rdfs:domain rdf:resource="techLayer1#Registry"/>
          <rdfs:range rdf:resource="http://www.w3.org/2001/XMLSchema#boolean"/>
          <rdfs:label>permissionless</rdfs:label>
          <rdfs:comment>Permissionless ledgers like Bitcoin and Ethereum have opened the world's eyes to the tremendous potential of DLT.</rdfs:comment>
     </owl:DatatypeProperty>

     <owl:DatatypeProperty rdf:about="techLayer1#public">
          <rdfs:domain rdf:resource="techLayer1#Registry"/>
          <rdfs:range rdf:resource="http://www.w3.org/2001/XMLSchema#boolean"/>
          <rdfs:label>public</rdfs:label>
          <rdfs:comment></rdfs:comment>
     </owl:DatatypeProperty>

     <owl:DatatypeProperty rdf:about="techLayer1#private">
          <rdfs:domain rdf:resource="techLayer1#Registry"/>
          <rdfs:range rdf:resource="http://www.w3.org/2001/XMLSchema#boolean"/>
          <rdfs:label>private</rdfs:label>
          <rdfs:comment></rdfs:comment>
     </owl:DatatypeProperty>



     <!-- ******************************* -->
     <!-- ********* Relation ************ -->
     <!-- ******************************* -->

     <owl:ObjectProperty rdf:about="techLayer1#hasArchitectureType">
          <rdfs:domain rdf:resource="techLayer1#Registry"/>
          <rdfs:range rdf:resource="techLayer1#ArchitectureType"/>
          <rdfs:label>has</rdfs:label>
          <rdfs:comment>Specifies the type of architecture used by a registry (centralized, decentralized, federated).</rdfs:comment>
          <rdfs:isDefinedBy rdf:resource="https://trustoverip.org/permalink/ToIP-Technical-Architecture-Specification-V1.0-PR1-2022-11-14.pdf"/>
     </owl:ObjectProperty>

     <owl:ObjectProperty rdf:about="techLayer1#reliesOnCentralizedRegistry">
          <rdfs:domain rdf:resource="techLayer1#CentralizedIdentifier"/>
          <rdfs:range rdf:resource="techLayer1#CentralizedArchitecture"/>
          <rdfs:label>relies on</rdfs:label>
          <rdfs:comment>The centraliazed identifier relies on a centralized architecture.</rdfs:comment>
          <rdfs:isDefinedBy rdf:resource="https://trustoverip.org/permalink/ToIP-Technical-Architecture-Specification-V1.0-PR1-2022-11-14.pdf"/>
     </owl:ObjectProperty>

     <owl:ObjectProperty rdf:about="techLayer1#supportsDecentralizedIdentifier">
          <rdfs:domain rdf:resource="techLayer1#DecentralizedArchitecture"/>
          <rdfs:range rdf:resource="techLayer1#DecentralizedIdentifier"/>
          <rdfs:label>supports</rdfs:label>
          <rdfs:comment>The decentraliazed architecture supports decentralized identifiers.</rdfs:comment>
          <rdfs:isDefinedBy rdf:resource="https://trustoverip.org/permalink/ToIP-Technical-Architecture-Specification-V1.0-PR1-2022-11-14.pdf"/>
     </owl:ObjectProperty>

     <owl:ObjectProperty rdf:about="techLayer1#rotatesIdentifier">
          <rdfs:domain rdf:resource="techLayer1#Identifier"/>
          <rdfs:range rdf:resource="techLayer1#Identifier"/>
          <rdfs:label>rotates</rdfs:label>
          <rdfs:comment>A ToIP identifier SHOULD support rotation of the associated cryptographic keys for the lifetime of the identifier. [L2.6] and section 8.2</rdfs:comment>
          <rdfs:isDefinedBy rdf:resource="https://trustoverip.org/permalink/ToIP-Technical-Architecture-Specification-V1.0-PR1-2022-11-14.pdf"/>
     </owl:ObjectProperty>

     <owl:ObjectProperty rdf:about="techLayer1#containsIdentifier">
          <rdfs:domain rdf:resource="techLayer1#Metadata"/>
          <rdfs:range rdf:resource="techLayer1#Identifier"/>
          <rdfs:label>contains</rdfs:label>
          <rdfs:comment>The metadata may contain the identifier (for example a X.509 certificate contains the public key in the PKI).</rdfs:comment>
          <rdfs:isDefinedBy rdf:resource=""/>
     </owl:ObjectProperty>

     <owl:ObjectProperty rdf:about="techLayer1#maintainsIdentifier">
          <rdfs:domain rdf:resource="techLayer1#Registry"/>
          <rdfs:range rdf:resource="techLayer1#Identifier"/>
          <rdfs:label>maintains</rdfs:label>
          <rdfs:comment>The registry verifies the identifier. [from Drummond Reed speech]</rdfs:comment>
          <rdfs:isDefinedBy rdf:resource="https://www.youtube.com/watch?v=2iB2HLgkjUw"/>
     </owl:ObjectProperty>

     <owl:ObjectProperty rdf:about="techLayer1#storesMetadata">
          <rdfs:domain rdf:resource="techLayer1#VDR"/>
          <rdfs:range rdf:resource="techLayer1#Metadata"/>
          <rdfs:label>stores</rdfs:label>
          <rdfs:comment>A registry that facilitates the creation, verification, updating, and/or deactivation of decentralized identifiers and DID documents. A verifiable data registry may also be used for other cryptographically-verifiable data structures such as verifiable credentials.</rdfs:comment>
          <rdfs:isDefinedBy rdf:resource="https://glossary.trustoverip.org/#term:registry"/>
     </owl:ObjectProperty>

     <owl:ObjectProperty rdf:about="techLayer1#resolvesRegistry">
          <rdfs:domain rdf:resource="techLayer1#Registry"/>
          <rdfs:range rdf:resource="techLayer1#Registry"/>
          <rdfs:label>resolves</rdfs:label>
          <rdfs:comment>A (meta)registry points to other (meta)registries for interoperability across systems.</rdfs:comment>
          <rdfs:isDefinedBy rdf:resource="http://ayra.forum/wp-content/uploads/2025/01/Ayra-Technical-Whitepaper-v0.0.10.pdf"/>
     </owl:ObjectProperty>



     <!-- ******************************* -->
     <!-- * Connection with other Layer * -->
     <!-- ******************************* -->

     <owl:Class rdf:about="techLayer4#Entity">
          <rdfs:label>Entity</rdfs:label>
          <rdfs:comment>Someone or something that is known to exist.</rdfs:comment>
          <rdfs:isDefinedBy rdf:resource="https://glossary.trustoverip.org/#term:entity"/>
     </owl:Class>

     <owl:Class rdf:about="techLayer3#Verifier">
          <rdfs:label>Verifier</rdfs:label>
          <rdfs:comment>A role an agent performs to perform verification of one or more proofs of the claims in a digital credential or other verifiable data.</rdfs:comment>
          <rdfs:isDefinedBy rdf:resource="https://glossary.trustoverip.org/#term:verifier"/>
     </owl:Class>

     <owl:Class rdf:about="techLayer3#Issuer">
          <rdfs:label>Issuer</rdfs:label>
          <rdfs:comment>A role an agent performs to package and digitally sign a set of claims, typically in the form of a digital credential, and transmit them to a holder.</rdfs:comment>
          <rdfs:isDefinedBy rdf:resource="https://glossary.trustoverip.org/#term:issuer"/>
     </owl:Class>

     <owl:ObjectProperty rdf:about="techLayer1#describesEntity">
          <rdfs:domain rdf:resource="techLayer1#Metadata"/>
          <rdfs:range rdf:resource="techLayer4#Entity"/>
          <rdfs:label>describes</rdfs:label>
          <rdfs:comment>Information describing the characteristics of data including, for example, structural metadata describing data structures (e.g., data format, syntax, and semantics) and descriptive metadata describing data contents (e.g., information security labels).</rdfs:comment>
          <rdfs:isDefinedBy rdf:resource="https://glossary.trustoverip.org/#term:metadata"/>
     </owl:ObjectProperty>

     <owl:ObjectProperty rdf:about="techLayer1#identifiesEntity">
          <rdfs:domain rdf:resource="techLayer1#Identifier"/>
          <rdfs:range rdf:resource="techLayer4#Entity"/>
          <rdfs:label>identifies</rdfs:label>
          <rdfs:comment>A single attribute—typically a character string—that uniquely identifies an entity within a specific context (which may be a global context). Examples include the name of a party, the URL of an organization, or a serial number for a man-made thing.</rdfs:comment>
          <rdfs:isDefinedBy rdf:resource="https://glossary.trustoverip.org/#term:verifiable-identifier"/>
     </owl:ObjectProperty>

     <owl:ObjectProperty rdf:about="techLayer3#issuerRegisteredInRegistry">
          <rdfs:domain rdf:resource="techLayer3#Issuer"/>
          <rdfs:range rdf:resource="techLayer1#Registry"/>
          <rdfs:label>registered in</rdfs:label>
          <rdfs:comment>The issuer is registered in the registry.</rdfs:comment>
          <rdfs:isDefinedBy rdf:resource="http://ayra.forum/wp-content/uploads/2025/01/Ayra-Technical-Whitepaper-v0.0.10.pdf"/>
     </owl:ObjectProperty>

     <owl:ObjectProperty rdf:about="techLayer3#verifierRegisteredInRegistry">
          <rdfs:domain rdf:resource="techLayer3#Verifier"/>
          <rdfs:range rdf:resource="techLayer1#Registry"/>
          <rdfs:label>registered in</rdfs:label>
          <rdfs:comment>The verifier is registered in the registry.</rdfs:comment>
          <rdfs:isDefinedBy rdf:resource="http://ayra.forum/wp-content/uploads/2025/01/Ayra-Technical-Whitepaper-v0.0.10.pdf"/>
     </owl:ObjectProperty>



     <!-- ******************************* -->
     <!-- ********* Instance ************ -->
     <!-- ******************************* -->



</rdf:RDF>
