<?xml version="1.0"?>
<rdf:RDF xmlns="http://example.org/techLayer1#"
     xml:base="http://example.org/techLayer1"
     xmlns:rdf="http://www.w3.org/1999/02/22-rdf-syntax-ns#"
     xmlns:owl="http://www.w3.org/2002/07/owl#"
     xmlns:rdfs="http://www.w3.org/2000/01/rdf-schema#"
     xmlns:xsd="http://www.w3.org/2001/XMLSchema#">

     <!-- ********************************************************************************************* -->
     <!-- *******************  All rights reserved to Cristian Lepore ********************************* -->
     <!-- ************************* Tech layer 1 of the ToIP model ************************************ -->
     <!-- ******** Definitions comes from the ToIP Glossary: https://glossary.trustoverip.org/ ******** -->
     <!-- ********************************************************************************************* -->

     <owl:Ontology rdf:about="http://example.org/techLayer1#">
          <rdfs:comment>Ontology representing the tech Layer 1 of the ToIP stack.</rdfs:comment>
     </owl:Ontology>



     <!-- ******************************* -->
     <!-- ********* Class *************** -->
     <!-- ******************************* -->

     <owl:Class rdf:about="techLayer1#TrustList">
          <rdfs:label>Trust List</rdfs:label>
          <rdfs:comment>A one-dimensional trust graph in which an authoritative source publishes a list of entities that are trusted in a specific trust context. A trust list can be considered a simplified form of a trust registry.</rdfs:comment>
          <rdfs:subClassOf rdf:resource="techLayer1#TrustRegistry"/>
          <rdfs:isDefinedBy rdf:resource="https://glossary.trustoverip.org/#term:trust-list"/>
     </owl:Class>

     <owl:Class rdf:about="techLayer1#VDR">
          <rdfs:label>VDR</rdfs:label>
          <rdfs:comment>A registry that facilitates the creation, verification, updating, and/or deactivation of decentralized identifiers and DID documents. A verifiable data registry may also be used for other cryptographically-verifiable data structures such as verifiable credentials.</rdfs:comment>
          <rdfs:subClassOf rdf:resource="techLayer1#Registry"/>
          <rdfs:isDefinedBy rdf:resource="https://glossary.trustoverip.org/#term:verifiable-data-registry"/>
     </owl:Class>

     <owl:Class rdf:about="techLayer1#ArchitectureType">
          <rdfs:label>Architecture type</rdfs:label>
          <rdfs:comment>The type of architecture of a registry.</rdfs:comment>
          <rdfs:isDefinedBy rdf:resource="https://trustoverip.org/permalink/ToIP-Technical-Architecture-Specification-V1.0-PR1-2022-11-14.pdf"/>
     </owl:Class>

     <owl:Class rdf:about="techLayer1#Federated">
          <rdfs:label>Federated</rdfs:label>
          <rdfs:comment>A group of organizations that collaborate to establish a common trust framework or governance framework for the exchange of identity data in a federated identity system.</rdfs:comment>
          <rdfs:subClassOf rdf:resource="techLayer1#ArchitectureType"/>
          <rdfs:isDefinedBy rdf:resource="https://glossary.trustoverip.org/#term:federation"/>
     </owl:Class>



     <!-- ******************************* -->
     <!-- ********* Attribute *********** -->
     <!-- ******************************* -->

     <owl:DatatypeProperty rdf:about="techLayer1#discoverable">
          <rdfs:domain rdf:resource="techLayer1#VID"/>
          <rdfs:range rdf:resource="http://www.w3.org/2001/XMLSchema#boolean"/>
          <rdfs:label>discoverable</rdfs:label>
          <rdfs:comment>A verifiable identifier may be discoverable. [L2.8]</rdfs:comment>
          <rdfs:isDefinedBy rdf:resource="https://trustoverip.org/permalink/ToIP-Technical-Architecture-Specification-V1.0-PR1-2022-11-14.pdf"/>
     </owl:DatatypeProperty>

     <owl:DatatypeProperty rdf:about="techLayer1#public">
          <rdfs:domain rdf:resource="techLayer1#Registry"/>
          <rdfs:range rdf:resource="http://www.w3.org/2001/XMLSchema#boolean"/>
          <rdfs:label>public</rdfs:label>
          <rdfs:comment></rdfs:comment>
     </owl:DatatypeProperty>



     <!-- ******************************* -->
     <!-- ********* Relation ************ -->
     <!-- ******************************* -->

     <owl:ObjectProperty rdf:about="techLayer1#containsIdentifier">
          <rdfs:domain rdf:resource="techLayer1#Metadata"/>
          <rdfs:range rdf:resource="techLayer1#Identifier"/>
          <rdfs:label>contains</rdfs:label>
          <rdfs:comment>The metadata may contain the identifier (for example a X.509 certificate contains the public key in the PKI).</rdfs:comment>
          <rdfs:isDefinedBy rdf:resource=""/>
     </owl:ObjectProperty>

     <owl:ObjectProperty rdf:about="techLayer1#maintainsIdentifier">
          <rdfs:domain rdf:resource="techLayer1#Registry"/>
          <rdfs:range rdf:resource="techLayer1#Identifier"/>
          <rdfs:label>maintains</rdfs:label>
          <rdfs:comment>The registry verifies the identifier. [from Drummond Reed speech]</rdfs:comment>
          <rdfs:isDefinedBy rdf:resource="https://www.youtube.com/watch?v=2iB2HLgkjUw"/>
     </owl:ObjectProperty>



     <!-- ******************************* -->
     <!-- * Connection with other Layer * -->
     <!-- ******************************* -->

     <owl:Class rdf:about="techLayer4#Entity">
          <rdfs:label>Entity</rdfs:label>
          <rdfs:comment>Someone or something that is known to exist.</rdfs:comment>
          <rdfs:isDefinedBy rdf:resource="https://glossary.trustoverip.org/#term:entity"/>
     </owl:Class>

     <owl:ObjectProperty rdf:about="techLayer3#issuerRegisteredInRegistry">
          <rdfs:domain rdf:resource="techLayer3#Issuer"/>
          <rdfs:range rdf:resource="techLayer1#Registry"/>
          <rdfs:label>registered in</rdfs:label>
          <rdfs:comment>The issuer is registered in the registry.</rdfs:comment>
          <rdfs:isDefinedBy rdf:resource="http://ayra.forum/wp-content/uploads/2025/01/Ayra-Technical-Whitepaper-v0.0.10.pdf"/>
     </owl:ObjectProperty>




     <!-- ******************************* -->
     <!-- ********* Instance ************ -->
     <!-- ******************************* -->



</rdf:RDF>
